refactor

theories/Assert.v
@@ -11,11 +11,11 @@ Unset Strict Implicit.
 Import Prenex Implicits.
 
 Definition setoid (p: trace -> Prop) :=
-forall tr0, p tr0 -> forall tr1, bisim tr0 tr1 -> p tr1.
+  forall tr0, p tr0 -> forall tr1, bisim tr0 tr1 -> p tr1.
 Definition assertS := state -> Prop.
-Definition assertT := { p: trace -> Prop | setoid p}.
+Definition assertT := {p: trace -> Prop | setoid p}.
 
-Definition assertS_and (u1 u2: assertS) := fun st =>  u1 st /\ u2 st.
+Definition assertS_and (u1 u2: assertS) := fun st => u1 st /\ u2 st.
 
 Infix "andS" := assertS_and (at level 60, right associativity).
 
@@ -44,155 +44,159 @@ Definition assertS_imp (u1 u2: assertS) := forall st, u1 st -> u2 st.
 Infix "->>" := assertS_imp (at level 60, right associativity).
 
 Lemma assertS_imp_refl: forall u, u ->> u.
-Proof.
-by move => u st0 h0.
-Qed.
+Proof. by move=>u. Qed.
 
-Definition satisfy (p:assertT) (tr: trace): Prop :=
-let: exist f0 h0 := p in f0 tr.
+Lemma impS_conseq_L: forall p0 p1 q,
+  p0 ->> p1 -> p1 ->> q -> p0 ->> q.
+Proof. move=>p0 p1 q h0 h1 st hst. by apply/h1/h0. Qed.
+
+Definition satisfy (p: assertT) (tr: trace): Prop :=
+  let: exist f0 h0 := p in f0 tr.
 
 Definition assertT_imp (p1 p2: assertT) :=
-forall tr, satisfy p1 tr -> satisfy p2 tr.
+  forall tr, satisfy p1 tr -> satisfy p2 tr.
 
 Infix "=>>" := assertT_imp (at level 60, right associativity).
 
 Lemma impT_conseq_L: forall p0 p1 q,
-p0 =>> p1 -> p1 =>> q -> p0 =>> q.
+  p0 =>> p1 -> p1 =>> q -> p0 =>> q.
 Proof.
 move=> [p0 hp0] [p1 hp1] [q hq] h0 h1 tr0 /= h2.
 by apply: h1=>/=; apply: h0=>/=.
 Qed.
 
 Lemma impT_conseq_R: forall p q0 q1,
-q0 =>> q1 -> p =>> q0 -> p =>> q1.
+  q0 =>> q1 -> p =>> q0 -> p =>> q1.
 Proof.
 move=>[p hp] [q0 hq0] [q1 hq1] h0 h1 tr0 /= h2.
 by apply: h0=>/=; apply: h1=>/=.
 Qed.
 
 Lemma imp_andT: forall p q0 q1,
-p =>> q0 -> p =>> q1 -> p =>> (q0 andT q1).
+  p =>> q0 -> p =>> q1 -> p =>> (q0 andT q1).
 Proof.
 move => [p hp] [q0 hq0] [q1 hq1] h0 h1 tr0 /= h2.
 by split; [apply: h0|apply: h1].
 Qed.
 
-Definition ttS: assertS := fun st => True.
-Definition ffS: assertS := fun st => False.
+Definition ttS: assertS := fun => True.
+Definition ffS: assertS := fun => False.
 
-Definition ttt: trace -> Prop := fun tr => True.
+Definition ttt: trace -> Prop := fun => True.
 Definition ttT: assertT.
-exists ttt. by move => tr0 h0 tr1 h1.
+by exists ttt.
 Defined.
 
 Lemma assertT_imp_refl: forall p, p =>> p.
-Proof. by move => p tr0 h0. Qed.
+Proof. by move => p. Qed.
 
 Lemma satisfy_cont: forall p0 p1,
- p0 =>> p1 -> forall tr, satisfy p0 tr -> satisfy p1 tr.
+  p0 =>> p1 -> forall tr, satisfy p0 tr -> satisfy p1 tr.
 Proof.
-move=> [f0 h0] [f1 h1] h2 tr /= h3. by apply: (h2 _ h3).
+move=> [f0 h0] [f1 h1] h2 tr /= h3. by apply: h2.
 Qed.
 
+(*
 Lemma assertT_imp_trans: forall p q r, p =>> q -> q =>> r -> p =>> r.
 Proof.
 move => p q r h0 h1 tr0 h2.
 by apply/(satisfy_cont h1)/(satisfy_cont h0).
 Qed.
+*)
 
 Lemma andS_left: forall u1 u2, (u1 andS u2) ->> u1.
-Proof. move => u1 u2 st h1; by inversion h1. Qed.
+Proof. by move => u1 u2 st [h1 _]. Qed.
 
 Lemma andS_right: forall u1 u2, (u1 andS u2) ->> u2.
-Proof. move => u1 u2 st h1; by inversion h1. Qed.
+Proof. by move => u1 u2 st [_ h2]. Qed.
+
+Lemma andS_comm: forall u1 u2, (u1 andS u2) ->> (u2 andS u1).
+Proof. by move=>u1 u2 st [h1]h2. Qed.
 
 Lemma andS_cont: forall u1 u1' u2 u2',
-u1 ->> u1' ->
-u2 ->> u2' ->
-(u1 andS u2) ->> (u1' andS u2').
+  u1 ->> u1' ->
+  u2 ->> u2' ->
+  (u1 andS u2) ->> (u1' andS u2').
 Proof.
 move => u1 u1' u2 u2' h1 h2 st [h3 h4].
 by split; [apply: (h1 _ h3)|apply: (h2 _ h4)].
 Qed.
 
-Lemma orT_left: forall p1 p2, p1 =>> (p1 orT p2).
-Proof.
-move => [f1 hf1] [f2 hf2] tr /= h1. by left.
-Qed.
+Lemma orT_left: forall p1 p2, p1 =>> p1 orT p2.
+Proof. by move => [f1 hf1] [f2 hf2] tr /= h1; left. Qed.
 
-Lemma orT_right: forall p1 p2, p2 =>> (p1 orT p2).
-Proof.
-move => [f1 hf1] [f2 hf2] tr /= h1. by right.
-Qed.
+Lemma orT_right: forall p1 p2, p2 =>> p1 orT p2.
+Proof. by move => [f1 hf1] [f2 hf2] tr /= h1; right. Qed.
 
-Definition singleton (u:assertS): trace -> Prop :=
-fun tr => exists st, u st /\ bisim tr (Tnil st).
+Definition singleton (u: assertS): trace -> Prop :=
+  fun tr => exists st, u st /\ bisim tr (Tnil st).
+
+Lemma singleton_nil: forall u st,
+  singleton u (Tnil st) -> u st.
+Proof. move => u st [st0 [h0 h1]]. by inv h1. Qed.
+
+Lemma mk_singleton_nil: forall (u : assertS) st,
+  u st -> singleton u (Tnil st).
+Proof. move => u st h0. by exists st; split=>//; apply bisim_nil. Qed.
 
 Lemma singleton_setoid: forall u, setoid (singleton u).
 Proof.
-move => u tr0 [st0 [h0 h2]] tr1 h1.
-inv h2. inv h1. exists st0.
-by split; [apply: h0 | apply: bisim_reflexive].
+move => u tr0 [st0][h0 h2] tr1 h1.
+inv h2. inv h1.
+by exact: mk_singleton_nil.
 Qed.
 
 Lemma singleton_monotone: forall u v, u ->> v ->
-forall tr, singleton u tr ->  singleton v tr.
+  forall tr, singleton u tr -> singleton v tr.
 Proof.
 move => u v huv tr0 [st0 [h0 h1]]. inv h1.
-exists st0.
-by split; [ apply: (huv _ h0) | apply: bisim_reflexive].
+by apply/mk_singleton_nil/huv.
 Qed.
-
-Lemma singleton_nil: forall u st,
-singleton u (Tnil st) -> u st.
-Proof. move => u st [st0 [h0 h1]]. by inv h1. Qed.
-
-Lemma mk_singleton_nil: forall (u : state -> Prop) st,
-u st -> singleton u (Tnil st).
-Proof. move => u st h0. exists st. split=>//; apply bisim_reflexive. Qed.
 
 (* Proposition 3.1: <U> is setoid *)
 Definition Singleton (u: assertS): assertT.
 exists (singleton u).
 move => tr0 [st0 [h0 h1]] tr1 h2. inv h1. inv h2.
-exists st0. by split=>//; apply: bisim_nil.
+by exact: mk_singleton_nil.
 Defined.
 
 Notation "[| p |]" := (Singleton p) (at level 80).
 
 (* Proposition 3.2: <U> is monotone *)
 Lemma Singleton_monotone: forall u v,
-u ->> v -> [|u|] =>> [|v|].
+  u ->> v -> [|u|] =>> [|v|].
 Proof.
-move => u v h0 tr0 [st0 [h1 h2]].
-inv h2. exists st0.
-by split; [ apply: (h0 _ h1) | apply: bisim_reflexive].
+move => u v h0 tr0 [st0 [h1 h2]]. inv h2.
+by apply/mk_singleton_nil/h0.
 Qed.
 
-Definition eval_true (a: expr): assertS  :=
-fun st => is_true (a st).
+Definition eval_true (a: expr): assertS :=
+  fun st => is_true (a st).
 
 Definition eval_false (a: expr): assertS :=
-fun st => ~~ is_true (a st).
+  fun st => ~~ is_true (a st).
 
 Definition dup (u: assertS): trace -> Prop :=
-fun tr => exists st, u st /\ bisim tr (Tcons st (Tnil st)).
+  fun tr => exists st, u st /\ bisim tr (Tcons st (Tnil st)).
+
+Lemma mk_dup: forall (u : assertS) st,
+  u st -> dup u (Tcons st (Tnil st)).
+Proof. move=>u st h. by exists st; split=>//; apply: bisim_reflexive. Qed.
 
 Lemma dup_cont: forall (u0 u1: assertS),
-u0 ->> u1 ->
-forall tr, dup u0 tr -> dup u1 tr.
+  u0 ->> u1 ->
+  forall tr, dup u0 tr -> dup u1 tr.
 Proof.
 move => u0 u1 hu tr [st0 [h0 h1]]. inv h1. inv H1.
-exists st0.
-by split; [apply: (hu _ h0)|apply: bisim_reflexive].
+by exists st0; split; [apply: hu | apply: bisim_reflexive].
 Qed.
 
 (* Proposition 3.1: <<U>> is setoid *)
 Definition Dup (u: assertS): assertT.
 exists (dup u).
 move => tr0 [st0 [h0 h1]] tr1 h2.
-inv h1. inv H1. inv h2. inv H2. exists st0.
-by split =>//; apply: bisim_reflexive.
+inv h1. inv H1. inv h2. inv H2.
+by exact: mk_dup.
 Defined.
 
 Notation "<< p >>" := (Dup p) (at level 80).
@@ -209,100 +213,94 @@ CoInductive follows (p: trace -> Prop): trace -> trace -> Prop :=
   follows p tr tr' -> follows p (Tcons st tr) (Tcons st tr').
 
 Lemma follows_hd: forall p tr0 tr1, follows p tr0 tr1 ->
-hd tr0 = hd tr1.
-Proof.
-move => p tr0 tr1 h0. by inv h0; simpl.
-Qed.
+  hd tr0 = hd tr1.
+Proof. move => p tr0 tr1 h0. by inv h0. Qed.
 
 Lemma follows_setoid: forall (p: trace -> Prop)
-(hp: forall tr0, p tr0 -> forall tr1, bisim tr0 tr1 -> p tr1),
-forall tr0 tr1, follows p tr0 tr1 ->
-forall tr2, bisim tr0 tr2 -> forall tr3, bisim tr1 tr3 ->
-follows p tr2 tr3.
+  (hp: forall tr0, p tr0 -> forall tr1, bisim tr0 tr1 -> p tr1),
+  forall tr0 tr1, follows p tr0 tr1 ->
+  forall tr2, bisim tr0 tr2 -> forall tr3, bisim tr1 tr3 ->
+  follows p tr2 tr3.
 Proof.
 move => p hp.
 cofix CIH => tr0 tr1 h0 tr2 h1 tr3 h2. inv h0.
-- clear CIH. inv h1.
-  have h0 := bisim_hd h2. symmetry in h0.
-  by apply: (follows_nil h0 (hp _ H0 _ h2)).
-- inv h2. inv h1. by apply: (follows_delay st (CIH _ _ H _ H4 _ H3)).
+- inv h1=>{CIH}.
+  apply: follows_nil; first by apply/esym/bisim_hd.
+  by apply/hp/h2.
+- inv h2. inv h1. by apply/follows_delay/CIH/H3/H4.
 Qed.
 
 Lemma follows_setoid_L: forall p,
-forall tr0 tr1, follows p tr0 tr1 ->
-forall tr2, bisim tr0 tr2 ->  follows p tr2 tr1.
+  forall tr0 tr1, follows p tr0 tr1 ->
+  forall tr2, bisim tr0 tr2 ->  follows p tr2 tr1.
 Proof.
 move => p. cofix CIH=>tr tr0 h0 tr1 h1. inv h0; inv h1.
 - by apply: follows_nil.
-- by apply: (follows_delay st (CIH _ _ H _ H3)).
+- by apply/follows_delay/CIH/H3.
 Qed.
 
 Lemma follows_setoid_R: forall (p: trace -> Prop)
-(hp: forall tr0, p tr0 -> forall tr1, bisim tr0 tr1 -> p tr1),
-forall tr tr0, follows p tr tr0 ->
-forall tr1, bisim tr0 tr1 ->  follows p tr tr1.
+  (hp: forall tr0, p tr0 -> forall tr1, bisim tr0 tr1 -> p tr1),
+  forall tr tr0, follows p tr tr0 ->
+  forall tr1, bisim tr0 tr1 ->  follows p tr tr1.
 Proof.
-move => p hp.
-cofix CIH=> tr tr0 h0 tr1 h1. inv h0.
-- apply/follows_nil.
-  - by apply/esym/bisim_hd.
-  by apply: (hp _ H0 _ h1).
-- inv h1. by apply: (follows_delay st (CIH _ _  H _ H3)).
+move => p hp. cofix CIH=> tr tr0 h0 tr1 h1. inv h0.
+- apply: follows_nil; first by apply/esym/bisim_hd.
+  by apply/hp/h1.
+- inv h1. by apply/follows_delay/CIH/H3.
 Qed.
 
 Lemma follows_monotone: forall (p q : trace -> Prop),
-(forall tr, p tr -> q tr) ->
-forall tr0 tr1, follows p tr0 tr1 -> follows q tr0 tr1.
+  (forall tr, p tr -> q tr) ->
+  forall tr0 tr1, follows p tr0 tr1 -> follows q tr0 tr1.
 Proof.
 move => p q hpq. cofix CIH=> tr0 tr1 h0. inv h0.
-- apply: follows_nil => //. by apply: (hpq _ H0).
+- by apply/follows_nil/hpq.
 - by apply/follows_delay/CIH.
 Qed.
 
 (* Lemma 3.2 *)
 Lemma follows_singleton: forall u tr0 tr1,
-follows (singleton u) tr0 tr1 -> bisim tr0 tr1.
+  follows (singleton u) tr0 tr1 -> bisim tr0 tr1.
 Proof.
 move => u. cofix CIH=> tr0 tr1 h0. inv h0.
-- move: H0 => [st0 [h0 h1]]. inv h1. by apply: bisim_reflexive.
-- by apply: (bisim_cons st (CIH _ _ H)).
+- move: H0 => [st0][h0 h1]. inv h1. by apply: bisim_reflexive.
+- by apply/bisim_cons/CIH.
 Qed.
 
 Lemma follows_singleton_andS_L: forall u0 u1 tr0,
-follows (singleton (u0 andS u1)) tr0 tr0 ->
-follows (singleton u0) tr0 tr0.
+  follows (singleton (u0 andS u1)) tr0 tr0 ->
+  follows (singleton u0) tr0 tr0.
 Proof.
 move => u0 u1. cofix CIH. case=> st0.
-- move =>h0. inversion h0. clear H1 H. simpl in H0.
-  inv h0.
-  move: H3 => [st1 [h1 h2]]. inv h2. move: h1 => [h1 h2].
-  apply follows_nil => //. exists st1. by split=>//; apply: bisim_reflexive.
+- move =>h0. inversion h0 => {H1 H H0}. inv h0=>{H0}.
+  move: H1 => [st1][[h1 h2] h3]. inv h3.
+  by apply/follows_nil/mk_singleton_nil.
 - move => tr0 h0. inv h0.
   by apply/follows_delay/CIH.
 Qed.
 
 Lemma follows_singleton_andS_R: forall u0 u1 tr0,
-follows (singleton (u0 andS u1)) tr0 tr0 ->
-follows (singleton u1) tr0 tr0.
+  follows (singleton (u0 andS u1)) tr0 tr0 ->
+  follows (singleton u1) tr0 tr0.
 Proof.
-move => u0 u1. cofix CIH. case.
-- move => st0 h0. inversion h0=>{H1 H}. simpl in H0.
-  inv h0.
-  move: H3 => [st1 [h1 h2]]. inv h2. move: h1 => [h1 h2].
-  apply follows_nil => //. exists st1. by split=>//; apply: bisim_reflexive.
-- move => st0 tr0 h0. inv h0.
-  by apply: (follows_delay st0 (CIH _ H0)).
+move => u0 u1. cofix CIH. case=>st0.
+- move => h0. inversion h0=>{H1 H H0}. inv h0=>{H0}.
+  move: H1 => [st1][[h1 h2] h3]. inv h3.
+  by apply/follows_nil/mk_singleton_nil.
+- move => tr0 h0. inv h0.
+  by apply/follows_delay/CIH.
 Qed.
 
 Lemma singleton_andS_follows: forall u v tr,
-follows (singleton u) tr tr -> follows (singleton v) tr tr ->
-follows (singleton (u andS v)) tr tr.
+  follows (singleton u) tr tr -> follows (singleton v) tr tr ->
+  follows (singleton (u andS v)) tr tr.
 Proof.
 move => u v. cofix CIH=> tr h0 h1. inversion h0; subst.
-- apply follows_nil => //. exists st. split; last by apply: bisim_reflexive.
-  clear H. inversion h1; subst. clear H1.
-  by split; [exact: singleton_nil H0|exact: singleton_nil H2].
-- subst. inv h0. inv h1. by apply: (follows_delay st (CIH _ H1 H2)).
+- apply/follows_nil/mk_singleton_nil => // {H}.
+  inv h1 => {H1}.
+  by split; exact: singleton_nil.
+- inv h0. inv h1. by apply/follows_delay/CIH.
 Qed.
 
 CoFixpoint lastdup (tr: trace): trace :=
@@ -312,100 +310,91 @@ match tr with
 end.
 
 Lemma lastdup_hd: forall tr, hd tr = hd (lastdup tr).
-Proof.
-case=>st.
-- by rewrite [lastdup _]trace_destr /=.
-- move => tr. by rewrite [lastdup _]trace_destr /=.
-Qed.
+Proof. case=>[?|??]; by rewrite [lastdup _]trace_destr /=. Qed.
 
 Lemma follows_dup: forall u tr, follows (singleton u) tr tr ->
-follows (dup u) tr (lastdup tr).
+  follows (dup u) tr (lastdup tr).
 Proof.
 move => u. cofix CIH=> tr0 h0. inversion h0.
 - clear H H1 H2 h0. rewrite [lastdup _]trace_destr /=.
-  move: H0 => [st1 [h0 h1]]. inv h1. apply follows_nil => //. exists st1.
-  by split=>//; apply: bisim_reflexive.
+  move: H0 => [st1 [h0 h1]]. inv h1.
+  by apply/follows_nil/mk_dup.
 - clear h0 H0 H. rewrite [lastdup _]trace_destr /=.
-  by apply: (follows_delay st (CIH _ H1)).
+  by apply/follows_delay/CIH.
 Qed.
 
 Definition append (p1 p2: trace -> Prop ): trace -> Prop :=
-fun tr => exists tr', p1 tr' /\ follows p2 tr' tr.
+  fun tr => exists tr', p1 tr' /\ follows p2 tr' tr.
 
 Infix "*+*" := append (at level 60, right associativity).
 
 Lemma append_cont: forall (p0 p1 q0 q1: trace -> Prop),
-(forall tr, p0 tr -> p1 tr) ->
-(forall tr, q0 tr -> q1 tr) ->
-forall tr, append p0 q0 tr -> append p1 q1 tr.
+  (forall tr, p0 tr -> p1 tr) ->
+  (forall tr, q0 tr -> q1 tr) ->
+  forall tr, append p0 q0 tr -> append p1 q1 tr.
 Proof.
 move => p0 p1 q0 q1 hp hq tr [tr0 [h0 h1]].
-exists tr0. split; first by apply: (hp _ h0).
+exists tr0. split; first by apply: hp.
 clear h0.
 move: tr0 tr h1. cofix CIH=> tr0 tr1 h0. inv h0.
-- apply follows_nil => //. by apply: (hq _ H0).
+- by apply/follows_nil/hq.
 - by apply/follows_delay/CIH.
 Qed.
 
 Lemma append_cont_L: forall (p0 p1 q: trace -> Prop),
-(forall tr, p0 tr -> p1 tr) ->
-forall tr, (append p0 q tr) -> (append p1 q tr).
+  (forall tr, p0 tr -> p1 tr) ->
+  forall tr, (append p0 q tr) -> (append p1 q tr).
 Proof.
 move => p0 p1 q hp tr [tr0 [h0 h1]].
-exists tr0. by split=>//; apply: (hp _ h0).
+exists tr0. by split=>//; apply: hp.
 Qed.
 
 Lemma append_monotone_R: forall (p q0 q1: trace -> Prop),
-(forall tr, q0 tr -> q1 tr) ->
-forall tr, (append p q0 tr) -> (append p q1 tr).
-Proof.
-move => p q0 q1 hq. by apply: (@append_cont p p _ _ _ hq).
-Qed.
+  (forall tr, q0 tr -> q1 tr) ->
+  forall tr, (append p q0 tr) -> (append p q1 tr).
+Proof. move => p q0 q1 hq. by apply: append_cont. Qed.
 
 Lemma append_setoid: forall (p0 p1: trace -> Prop),
-setoid p1 -> setoid (append p0 p1).
+  setoid p1 -> setoid (append p0 p1).
 Proof.
 move => p0 p1 hp1 tr0 [tr2 [h0 h2]] tr1 h1.
-exists tr2. split; first by apply h0.
-by apply: (follows_setoid_R hp1 h2 h1).
+exists tr2. split; first by apply: h0.
+by apply/follows_setoid_R/h1.
 Qed.
 
 Lemma follows_follows: forall p q tr0 tr1 tr2, follows p tr0 tr1 ->
-follows q tr1 tr2 -> follows (p *+* q) tr0 tr2.
-Proof. move => p q. cofix CIH. case.
-- move => st0 tr1 tr2 h0 h1. inv h0.
-  have h2 := follows_hd h1.
-  apply follows_nil => //. by exists tr1.
-- move => st0 tr0 tr1 tr2 h0 h1. inv h0. inv h1.
-  by apply/follows_delay/(CIH _ _ _ H2).
+  follows q tr1 tr2 -> follows (p *+* q) tr0 tr2.
+Proof. move => p q. cofix CIH. case=>st0.
+- move => tr1 tr2 h0 h1. inv h0.
+  apply follows_nil; first by apply/esym/follows_hd/h1.
+  by exists tr1.
+- move => tr0 tr1 tr2 h0 h1. inv h0. inv h1.
+  by apply/follows_delay/CIH/H3.
 Qed.
 
 CoInductive midp (p0 p1: trace -> Prop) (tr0 tr1: trace) (h: follows (append p0 p1) tr0 tr1) : trace -> Prop :=
 | midp_follows_nil :
-   forall tr, tr0 = Tnil (hd tr1) -> p0 tr -> follows p1 tr tr1 -> midp h tr
+  forall tr, tr0 = Tnil (hd tr1) -> p0 tr -> follows p1 tr tr1 -> midp h tr
 | midp_follows_delay :
   forall (tr2 tr3 :trace) (h1: follows (append p0 p1) tr2 tr3) (st : state) tr',
   tr0 = Tcons st tr2 -> tr1 = Tcons st tr3 -> @midp p0 p1 tr2 tr3 h1 tr' ->
   midp h (Tcons st tr').
 
 Lemma midp_before: forall p0 p1 tr0 tr1 (h: follows (append p0 p1) tr0 tr1) tr',
-midp h tr' ->
-follows p0 tr0 tr'.
+  midp h tr' ->
+  follows p0 tr0 tr'.
 Proof.
-cofix CIH. dependent inversion h. move => {tr H0}.
-- move: tr1 st tr0 h e a H. case.
-  - move => st0 st1 tr0 h1 /= h2 h3 h4 tr' hm.
+cofix CIH. dependent inversion h.
+- move => {tr H0}; move: tr1 st tr0 h e a H. case=>st0.
+  - move => st1 tr0 h1 /= h2 h3 h4 tr' hm.
     inv hm; last by inversion H.
-    destruct h3. destruct H2. inversion h1.
-    subst. apply: follows_nil =>//.
-    by inversion H1.
-  - move => st0 tr0 st1 tr1 h1 /= h2 h3 h4 tr' hm.
+    destruct h3. destruct H2. inv h1.
+    apply: follows_nil =>//. by inversion H1.
+  - move => tr0 st1 tr1 h1 /= h2 h3 h4 tr' hm.
     inv hm; last by inversion H.
-    destruct h3. destruct H2. inversion h1.
-    subst. apply: follows_nil=>//. by inversion H1.
-- subst.
-  move => tr0 hm.
-  destruct tr0; first by inversion hm.
+    destruct h3. destruct H2. inv h1.
+    apply: follows_nil=>//. by inversion H1.
+- subst=> tr0 hm; destruct tr0; first by inversion hm.
   inv hm; subst; first by inversion H.
   inv H1; subst.
   inv H2; subst.
@@ -413,20 +402,19 @@ cofix CIH. dependent inversion h. move => {tr H0}.
 Qed.
 
 Lemma midp_after: forall p0 p1 tr0 tr1 (h: follows (append p0 p1) tr0 tr1) tr',
-midp h tr' ->
-follows p1 tr' tr1.
+  midp h tr' ->
+  follows p1 tr' tr1.
 Proof.
-cofix CIH. dependent inversion h. move => {tr H0}.
-- move: tr1 st tr0 h e a H. case.
-  * move => st0 st1 tr0 h1 /= h2 h3 h4 tr' hm.
-    inv hm; last by inversion H. destruct tr'; last by inversion H.
-    destruct h3. destruct H2. inversion H3. subst.
+cofix CIH. dependent inversion h.
+- move => {tr H0}; move: tr1 st tr0 h e a H. case=>st0.
+  * move => st1 tr0 h1 /= h2 h3 h4 tr' hm.
+    inv hm; last by inversion H.
+    destruct tr'; last by inversion H.
+    destruct h3. destruct H2. inv H3.
     apply: follows_nil=>//. by inversion H1.
-  * move => st0 tr0 st1 tr1 h1 /= h2 h3 h4 tr' hm.
+  * move => tr0 st1 tr1 h1 /= h2 h3 h4 tr' hm.
     inv hm; by inversion H.
-subst.
-move => tr0 hm.
-destruct tr0; first by inversion hm.
+subst=> tr0 hm; destruct tr0; first by inversion hm.
 inv hm; subst; first by inversion H.
 inv H1; subst.
 inv H2; subst.
@@ -434,14 +422,14 @@ by apply/follows_delay/(CIH _ _ _ _ h1).
 Qed.
 
 Lemma append_assoc_L: forall p1 p2 p3 tr,
-(append (append p1 p2) p3) tr -> append p1 (append p2  p3) tr.
+  (append (append p1 p2) p3) tr -> append p1 (append p2 p3) tr.
 Proof.
-move => p1 p2 p3 tr0 [tr1 [[tr2 [h1 h3]] h2]].
+move => p1 p2 p3 tr0 [tr1][[tr2][h1 h3] h2].
 exists tr2. split=>// {h1}.
 move: tr2 tr0 tr1 h2 h3. cofix CIH=> tr0 tr1 tr2 h1 h2. inv h2.
 - apply/follows_nil; first by apply/esym/follows_hd/h1.
   by exists tr2.
-- inv h1. by apply/follows_delay/(CIH _ _ _ H3).
+- inv h1. by apply/follows_delay/CIH/H.
 Qed.
 
 (* Proposition 3.1: ** is setoid. *)
@@ -449,14 +437,14 @@ Definition Append (p1 p2: assertT): assertT.
 destruct p1 as [f0 h0]. destruct p2 as [f1 h1].
 exists (append f0 f1).
 move => tr0 [tr1 [h2 h3]] tr2 h4. exists tr1.
-split=>//. by apply: (follows_setoid_R h1 h3 h4).
+split=>//. by apply/follows_setoid_R/h4.
 Defined.
 
 Infix "***" := Append (at level 60, right associativity).
 
 (* Lemma 3.4 (4) => *)
 Lemma Append_assoc_L: forall p1 p2 p3,
-((p1 *** p2) *** p3) =>> (p1 *** p2 *** p3).
+  ((p1 *** p2) *** p3) =>> (p1 *** p2 *** p3).
 Proof.
 move => [f1 hf1] [f2 hf2] [f3 hf3] tr0 /= h1.
 by apply: append_assoc_L.
@@ -464,112 +452,115 @@ Qed.
 
 (* Proposition 3.2: ** is monotone *)
 Lemma Append_monotone: forall p1 p2 q1 q2,
-p1 =>> p2 -> q1 =>> q2 -> (p1 *** q1) =>> (p2 *** q2).
+  p1 =>> p2 -> q1 =>> q2 -> (p1 *** q1) =>> (p2 *** q2).
 Proof.
 move=> [p1 hp1] [p2 hp2] [q1 hq1] [q2 hq2] h0 h1 tr0 /= h2.
-by apply: (append_cont _ _ h2).
+by apply/append_cont/h2.
 Qed.
 
 Lemma Append_monotone_L: forall p1 p2 q,
-p1 =>> p2 -> (p1 *** q) =>> (p2 *** q).
+  p1 =>> p2 -> (p1 *** q) =>> (p2 *** q).
 Proof.
 move=> [p1 hp1] [p2 hp2] [q hq] h0 tr0 /=.
 by apply: append_cont_L.
 Qed.
 
 Lemma Append_monotone_R: forall q p1 p2,
-p1 =>> p2 -> (q *** p1) =>> (q *** p2).
+  p1 =>> p2 -> (q *** p1) =>> (q *** p2).
 Proof.
 move => [q hq] [p1 hp1] [p2 hp2] h0 tr0 /= h1.
-by apply: (@append_cont q q p1 p2).
+by apply/append_cont/h1.
+Qed.
+
+(* Lemma 3.1 *)
+Lemma follows_ttS: forall tr, follows (singleton ttS) tr tr.
+Proof.
+cofix CIH. case=> st0.
+- by apply/follows_nil/mk_singleton_nil.
+- move => tr0. by apply/follows_delay/CIH.
 Qed.
 
 Lemma Append_ttS: forall p,
-p =>> (p *** [| ttS |]).
+  p =>> (p *** [| ttS |]).
 Proof.
-move => [f hp] tr0 /= h0. exists tr0.
-split=>// {h0 hp}. move: tr0. cofix CIH. case=>st0.
-- apply: follows_nil => //; by apply mk_singleton_nil.
-move=>tr0.
-by apply/follows_delay/CIH.
+move => [f hp] tr0 /= h0.
+exists tr0. split=>// {h0 hp}.
+by exact: follows_ttS.
 Qed.
 
 (* Lemma 3.4 (1), the first => *)
 Lemma Sglt_Dup_1: forall u v, ([|u|] *** <<v>>) =>> <<u andS v>>.
 Proof.
-move=>u v tr0 [tr1 [[st0 [h0 h2]] h1]] /=. inv h2. inv h1.
-destruct H1 as [st0 [h1 h2]]. inv h2. inv H1. simpl in h0. exists st0.
-by split=>//; apply: bisim_reflexive.
+move=>u v tr0 [tr1][[st0][h0 h2] h1] /=. inv h2. inv h1.
+destruct H1 as [st0 [h1 h2]]. inv h2. inv H1. simpl in h0.
+by apply: mk_dup.
 Qed.
 
 (* Lemma 3.4 (1), the first <= *)
 Lemma Sglt_Dup_2: forall u v, <<u andS v>> =>> ([|u|] *** <<v>>).
 Proof.
-move => u v tr0 [st0 [[hu hv] h1]]. inv h1. inv H1. exists (Tnil st0). split.
-* exists st0. by split=>//; apply: bisim_reflexive.
-* apply follows_nil => //. exists st0. by split=>//; apply: bisim_reflexive.
+move => u v tr0 [st0 [[hu hv] h1]]. inv h1. inv H1.
+exists (Tnil st0); split; first by exact: mk_singleton_nil.
+by apply/follows_nil/mk_dup.
 Qed.
 
 (* Lemma 3.4 (1), the second => *)
 Lemma Sglt_Dup_3: forall u v, <<u andS v>> =>> <<u>> *** [|v|].
 Proof.
-move => u v tr0 [st0 [[hu hv] h0]]. inv h0. inv H1. exists (Tcons st0 (Tnil st0)).
-split.
-- exists st0. by split=>//; apply: bisim_reflexive.
-apply/follows_delay/follows_nil => //. exists st0.
-by split=>//; apply: bisim_reflexive.
+move => u v tr0 [st0 [[hu hv] h0]]. inv h0. inv H1.
+exists (Tcons st0 (Tnil st0)); split; first by exact: mk_dup.
+by apply/follows_delay/follows_nil/mk_singleton_nil.
 Qed.
 
 (* Lemma 3.4 (1), the second <= *)
 Lemma Sglt_Dup_4: forall u v, (<<u>> *** [|v|]) =>> <<u andS v>>.
 Proof.
-move => u v tr0 [tr1 [[st0 [hu h0]] h1]]. inv h0. inv H1.
-inv h1. inv H2. destruct H1 as [st0 [hv h0]]. inv h0. simpl in hu. simpl.
-exists st0. by split=>//; apply: bisim_reflexive.
+move => u v tr0 [tr1][[st0][hu h0] h1].
+inv h0. inv H1. inv h1. inv H2.
+destruct H1 as [st0 [hv h0]]. inv h0. simpl in hu. simpl.
+by apply: mk_dup.
 Qed.
 
 (* Lemma 3.4 (2), => *)
 Lemma Sglt_Chop_1: forall u v, ([|u|] *** [|v|]) =>> [|u andS v|].
 Proof.
-move => u v tr0 [tr1 [[st0 [hu h0]] h1]]. inv h0.
-inv h1. destruct H1 as [st0 [hv h0]]. inv h0. simpl in hu. exists st0.
-by split=>//; apply: bisim_reflexive.
+move => u v tr0 [tr1 [[st0 [hu h0]] h1]].
+inv h0. inv h1. destruct H1 as [st0 [hv h0]]. inv h0. simpl in hu. simpl.
+by apply: mk_singleton_nil.
 Qed.
 
 (* Lemma 3.4 (2), <= *)
 Lemma Sglt_Chop_2: forall u v, [|u andS v|] =>> [|u|] *** [|v|].
 Proof.
-move => u v tr0 [st0 [[hu hv] h0]]. inv h0. exists (Tnil st0).
-split.
-- exists st0. by split=>//; apply: bisim_reflexive.
-apply: follows_nil => //.
-exists st0. by split=>//; apply: bisim_reflexive.
+move => u v tr0 [st0 [[hu hv] h0]]. inv h0.
+exists (Tnil st0). split; first by exact: mk_singleton_nil.
+by apply/follows_nil/mk_singleton_nil.
 Qed.
 
 Lemma Singleton_Append: forall v p, ([|v|] *** p) =>> p.
 Proof.
-move => v [p hp] tr0 /= [tr1 [[st0 [h0 h2]] h1]].
-inv h2. by inv h1.
+move => v [p hp] tr0 /= [tr1][[st0][h0 h2] h1].
+by inv h2; inv h1.
 Qed.
 
 (* Lemma 3.4 (3), the first => *)
 Lemma ttS_Chop: forall p,
-([|ttS|] *** p) =>> p.
+  ([|ttS|] *** p) =>> p.
 Proof. move => p. by apply Singleton_Append. Qed.
 
 (* Lemma 3.4 (3), the first <= *)
 Lemma ttS_Chop_2: forall p,  p =>> [|ttS|] *** p.
 Proof.
-move => [p hp] tr0 /= htr0. exists (Tnil (hd tr0)). split.
-- exists (hd tr0). by split=>//; apply: bisim_reflexive.
+move => [p hp] tr0 /= htr0.
+exists (Tnil (hd tr0)). split; first by exact: mk_singleton_nil.
 by exact: follows_nil.
 Qed.
 
 Lemma append_singleton: forall p (hp: setoid p) u tr,
-append p (singleton u) tr -> p tr.
+  append p (singleton u) tr -> p tr.
 Proof.
-move => p hp u tr0 [tr1 [h1 h2]].
-by apply/(hp _ h1)/(follows_singleton h2).
+move => p hp u tr0 [tr1][h1 h2].
+by apply/hp/follows_singleton/h2.
 Qed.
 
 Lemma Append_Singleton: forall p v, (p *** [|v|]) =>> p.
@@ -582,10 +573,9 @@ Proof. move => p. by apply Append_Singleton. Qed.
 (* Lemma 3.4 (3), the second => *)
 Lemma Chop_ttS_2: forall p, p =>> p *** [|ttS|].
 Proof.
-move => [p hp] tr0 /= htr0. exists tr0; split=>// {hp htr0}.
-move: tr0. cofix CIH. case=>st0.
-- apply follows_nil=>//. exists st0. by split=>//; apply: bisim_reflexive.
-- by move=>tr0; apply/follows_delay/CIH.
+move => [p hp] tr0 /= htr0.
+exists tr0; split=>// {hp htr0}.
+by exact: follows_ttS.
 Qed.
 
 Lemma ttT_idem_comp: (ttT *** ttT) =>> ttT.
@@ -597,7 +587,7 @@ Inductive finite: trace -> Prop :=
   finite tr -> finite (Tcons st tr).
 
 Lemma finite_setoid: forall tr, finite tr ->
-forall tr0, bisim tr tr0 -> finite tr0.
+  forall tr0, bisim tr tr0 -> finite tr0.
 Proof.
 induction 1=>tr0 h0; inv h0.
 - by apply: finite_nil.
@@ -608,12 +598,12 @@ Qed.
 Definition Finite: assertT.
 exists (fun tr => finite tr).
 move => tr0 h0 tr1 h1.
-apply: (finite_setoid h0 h1).
+by apply/finite_setoid/h1.
 Defined.
 
 Lemma Finite_idem_1: (Finite *** Finite) =>> Finite.
 Proof.
-move => tr0 [tr1 [h0 h1]]. move: tr1 h0 tr0 h1. induction 1=>tr0.
+move => tr0 [tr1][h0 h1]. move: tr1 h0 tr0 h1. induction 1=>tr0.
 - move => h0. by inv h0.
 - move => h1. inv h1.
   by apply/finite_delay/IHh0.
@@ -628,7 +618,7 @@ Qed.
 Lemma Finite_singleton: forall u, (Finite *** [|u|]) =>> Finite.
 Proof.
 move => u tr /= [tr1 [h0 h1]].
-by apply/(finite_setoid h0)/follows_singleton/h1.
+by apply/finite_setoid/follows_singleton/h1.
 Qed.
 
 CoInductive iter (p: trace -> Prop): trace -> Prop :=
@@ -638,47 +628,53 @@ CoInductive iter (p: trace -> Prop): trace -> Prop :=
   follows (iter p) tr tr0 ->
   iter p tr0.
 
+Lemma follows_iter: forall p tr, follows (iter p) tr tr.
+Proof.
+move=>p. cofix CIH. case=>st.
+- by apply/follows_nil/iter_stop.
+- move => tr. by apply/follows_delay/CIH.
+Qed.
+
 Lemma iter_setoid: forall p (hp: setoid p), setoid (iter p).
 Proof.
 move => p hp. cofix CIH.
 have h0: forall tr, setoid (follows (iter p) tr).
-* cofix COINDHYP1=> tr tr0 h0 tr1 h1. inv h0.
+* cofix CIH1=> tr tr0 h0 tr1 h1. inv h0.
   - apply: follows_nil; first by apply/esym/bisim_hd.
     by apply: (CIH _ H0 _ h1).
-  - inv h1. by apply: (follows_delay st (COINDHYP1 _ _ H _ H3)).
-* move => tr0 h1 tr1 h2. inv h1.
-  - inv h2. by apply: iter_stop.
-  - by apply: (iter_loop H (h0 _ _ H0 _ h2)).
+  - inv h1. by apply/follows_delay/CIH1/H3.
+move => tr0 h1 tr1 h2. inv h1.
+- inv h2. by apply: iter_stop.
+- by apply/iter_loop/h0/h2/H0.
 Qed.
 
 Lemma iter_cont: forall (p0 p1: trace -> Prop),
-(forall tr, p0 tr -> p1 tr) ->
-forall tr, iter p0 tr -> iter p1 tr.
+  (forall tr, p0 tr -> p1 tr) ->
+  forall tr, iter p0 tr -> iter p1 tr.
 Proof.
 move => p0 p1 hp. cofix CIH.
 have h: forall tr0 tr1, follows (iter p0) tr0 tr1 -> follows (iter p1) tr0 tr1.
-* cofix COINDHYP0=> tr0 tr1 h0. inv h0.
-  - apply follows_nil=>//. by apply: CIH.
-  - by apply: (follows_delay st (COINDHYP0 _ _ H)).
-* move => tr0 h0. inv h0.
-  - apply iter_stop.
-  - by apply: (iter_loop (hp _ H)  (h _ _ H0)).
+* cofix CIH0=> tr0 tr1 h0. inv h0.
+  - by apply/follows_nil/CIH.
+  - by apply/follows_delay/CIH0.
+move => tr0 h0. inv h0.
+- by apply: iter_stop.
+- by apply/iter_loop/h/H0/hp.
 Qed.
 
 Lemma iter_append_dup: forall (u : state -> Prop) p tr,
-u (hd tr) -> iter (append p (dup u)) tr ->
-follows (singleton u) tr tr.
+  u (hd tr) -> iter (append p (dup u)) tr ->
+  follows (singleton u) tr tr.
 Proof.
 move => u p. cofix CIH=> tr h0 h1. inv h1.
-- simpl in h0. apply follows_nil => //. exists st.
-  by split=>//; apply: bisim_reflexive.
-- move: H => [tr1 [h2 h1]]. clear h2 h0. (*
-  have h2 := follows_hd X0.  rewrite -h2 in h0 => {h2}.   *)
+- by apply/follows_nil/mk_singleton_nil.
+- move: H => [tr1 [_ h1]] {h0}.
   move: tr tr1 tr0 h1 H0.
-  cofix hcoind1=> tr0 tr1 tr2 h0 h1. inv h0.
-  - move: H0 => [st0 [h0 h3]]. inv h3. inv H1.
-    inv h1. inv H2. by apply: (follows_delay _ (CIH _ h0 H1)).
-  - inv h1. by apply: (follows_delay _ (hcoind1 _ _ _ H H3)).
+  cofix CIH1=> tr0 tr1 tr2 h0 h1. inv h0.
+  - move: H0 => [st0 [h0 h3]].
+    inv h3. inv H1. inv h1. inv H2.
+    by apply/follows_delay/CIH.
+  - inv h1. by apply/follows_delay/CIH1/H3/H.
 Qed.
 
 (* Proposition 3.2: Iter is setoid. *)
@@ -691,22 +687,26 @@ Defined.
 Lemma Iter_monotone: forall p q, p =>> q -> (Iter p) =>> (Iter q).
 Proof.
 move => [p hp] [q hq] h0 tr0 /=.
-apply: iter_cont=> tr1. apply: h0.
+by apply/iter_cont/h0.
 Qed.
 
 Definition updt (u: assertS) (x:id) (a: expr): trace -> Prop :=
-fun tr => exists st, u st /\ bisim tr (Tcons st (Tnil (update x (a st) st))).
+  fun tr => exists st, u st /\ bisim tr (Tcons st (Tnil (update x (a st) st))).
+
+Lemma mk_updt: forall (u : assertS) x a st,
+  u st -> updt u x a (Tcons st (Tnil (update x (a st) st))).
+Proof. move=>u x a st h. by exists st; split=>//; apply: bisim_reflexive. Qed.
 
 (* Proposition 3.1: U[x↦e] is setoid. *)
 Definition Updt (u: assertS) (x:id) (a: expr): assertT.
 exists (updt u x a).
 move => tr0 [st0 [h0 h1]] tr1 h2.
-exists st0. inv h1. inv H1. inv h2. inv H2.
-by split=>//; apply: bisim_reflexive.
+inv h1. inv H1. inv h2. inv H2.
+by exact: mk_updt.
 Defined.
 
 Definition exS (A: Type) (u: A -> assertS) : assertS :=
-fun st => exists x, u x st.
+  fun st => exists x, u x st.
 
 Definition exT (A: Type) (p: A -> assertT) : assertT.
 exists (fun tr => exists x, satisfy (p x) tr).
@@ -718,7 +718,7 @@ Definition negT (p: assertT): assertT.
 destruct p as [f hf].
 exists (fun tr => f tr -> False).
 move => tr0 h0 tr1 h1 /= h2.
-by move: (hf _ h2 _ (bisim_symmetric h1)).
+by apply/h0/hf/bisim_symmetric/h1.
 Defined.
 
 CoInductive infinite: trace -> Prop :=
@@ -727,18 +727,19 @@ CoInductive infinite: trace -> Prop :=
 
 (* Proposition 3.1: Infinite is setoid. *)
 Definition Infinite: assertT.
-exists (fun tr => infinite tr).
+exists infinite.
 move => tr0 /= h0 tr1 h1.
 move: tr0 h0 tr1 h1. cofix CIH => tr0 h0 tr1 h1.
-inv h0. inv h1. by apply: (infinite_delay st (CIH _ H _ H3)).
+inv h0. inv h1.
+by apply/infinite_delay/CIH/H3.
 Defined.
 
 (* Lemma 3.4 (7), => *)
 Lemma infinite_implies_true_chop_false: Infinite =>> (ttT *** [|ffS|]).
 Proof.
 move => tr0 [st0 tr1] hinfinite /=. exists (Tcons st0 tr1). split => // {tr0}.
-move: st0 tr1 hinfinite.
-cofix hcofix=> st0 tr0 h. apply follows_delay. inversion h. subst.
+move: st0 tr1 hinfinite. cofix hcofix=> st0 tr0 h.
+apply follows_delay. inv h.
 by apply/hcofix/H.
 Qed.
 
@@ -746,32 +747,28 @@ Qed.
 Lemma true_chop_false_implies_infinite: (ttT *** [|ffS|]) =>> Infinite.
 Proof.
 move => tr0 [tr1 [_ h1]] /=.
-move: tr0 tr1 h1. cofix h0 => tr0 tr1 h1.
-inv h1.
+move: tr0 tr1 h1. cofix h0 => tr0 tr1 h1. inv h1.
 - destruct H0 as [st0 [h1 h2]]. by inversion h1.
-- by apply/infinite_delay/(h0 _ _ H).
+- by apply/infinite_delay/h0/H.
 Qed.
 
 (* extensions *)
 Lemma iter_split_1: forall p tr, iter p tr -> (singleton ttS tr) \/ (append p (iter p) tr).
 Proof.
 move => p tr h0. inv h0.
-- left. exists st. by split => //; apply: bisim_reflexive.
+- left. by exact: mk_singleton_nil.
 - right. by exists tr0.
 Qed.
 
 (* Lemma 3.4 (5), => *)
 Lemma Iter_unfold_0: forall p, Iter p =>> ([|ttS|] orT (p *** Iter p)).
-Proof.
-move => [p hp] tr0 /= h0.
-by apply: iter_split_1.
-Qed.
+Proof. move => [p hp] tr0 /= h0. by apply: iter_split_1. Qed.
 
 Lemma iter_split_2: forall tr p, (singleton ttS tr) \/ (append p (iter p) tr) -> iter p tr.
 Proof.
 move => tr p h. inv h.
 - move: H => [st [h0 h1]]. inv h1. by apply: iter_stop.
-- move: H => [tr0 [h0 h1]]. by apply: (iter_loop h0 h1).
+- move: H => [tr0 [h0 h1]]. by apply/iter_loop/h1.
 Qed.
 
 (* Lemma 3.4 (5), <= *)
@@ -782,15 +779,13 @@ Lemma iter_unfold_1: forall p tr, (iter p *+* p) tr -> iter p tr.
 Proof.
 move => p tr [tr0 [h0 h1]].
 move: tr0 tr h0 h1. cofix CIH=> tr0 tr1 h0 h1. inv h0.
-- inv h1. apply: (iter_loop H1) => {H1}. move: tr1. cofix CIH0.
-  case.
-  * move => st. apply: follows_nil => //. by apply: iter_stop.
-  move => st0 tr0. by apply/follows_delay/CIH0.
+- inv h1. apply: (iter_loop H1) => {H1}.
+  by exact: follows_iter.
 - apply: (iter_loop H) => {H}. move: tr tr0 tr1 H0 h1.
   cofix CIH0 => tr0 tr1 tr2 h0 h1. inv h0.
-  - have h0 := follows_hd h1. apply follows_nil => //.
-    by apply: (CIH _ _ H0 h1).
-  - inv h1. by apply/follows_delay/(CIH0 _ _ _ H H3).
+  - apply follows_nil; first by apply/esym/follows_hd/h1.
+    by apply/CIH/h1.
+  - inv h1. by apply/follows_delay/CIH0/H3.
 Qed.
 
 Lemma Iter_unfold_1: forall p, (Iter p *** p) =>> Iter p.
@@ -809,7 +804,7 @@ Qed.
 Lemma Stop_Iter: forall p, [|ttS|] =>> Iter p.
 Proof.
 move => [p hp] /= t0 h0. inv h0.
-move: H => [_ h0]. inv h0. simpl. by apply: iter_stop.
+move: H => [_ h0]. inv h0. by apply: iter_stop.
 Qed.
 
 Lemma Iter_fold_L: forall p, (p *** Iter p) =>> Iter p.
@@ -821,9 +816,7 @@ Qed.
 Lemma iter_iter_2: forall p tr, iter p tr -> append (iter p) (iter p) tr.
 Proof.
 move => p tr0 h0. exists tr0. split => // {h0}. move: tr0.
-cofix CIH. case=> st0.
-- apply follows_nil => //. by apply iter_stop.
-- move => tr0. by apply/follows_delay/CIH.
+by exact: follows_iter.
 Qed.
 
 (* Lemma 3.4 (6), => *)
@@ -837,56 +830,47 @@ cofix CIH=> tr0 tr1 h0. inv h0=>h0.
 - by inv h0.
 - apply: (iter_loop H) => {H}. move: tr tr0 tr1 H0 h0.
   cofix CIH2=> tr0 tr1 tr2 h0. inv h0=>h0.
-  - apply: follows_nil; first by apply/esym/(follows_hd h0).
-    by apply: (CIH _ _ H0).
-  - inv h0. by apply/follows_delay/(CIH2 _ _ _ H).
+  - apply: follows_nil; first by apply/esym/follows_hd/h0.
+    by apply/CIH/h0.
+  - inv h0. by apply/follows_delay/CIH2/H3.
 Qed.
 
 (* Lemma 3.4. (6), <= *)
 Lemma Iter_Iter: forall p, (Iter p *** Iter p) =>> Iter p.
 Proof. move => [p hp] tr /=. by apply: iter_iter. Qed.
 
-(* Lemma 3.1 *)
-Lemma follows_ttS: forall tr, follows (singleton ttS) tr tr.
-Proof.
-cofix CIH. case=> st0.
-- apply follows_nil => //. exists st0.
-  by split => //; apply: bisim_reflexive.
-- move => tr0. by apply/follows_delay/CIH.
-Qed.
-
 Inductive fin: trace -> state -> Prop :=
 | fin_nil: forall st, fin (Tnil st) st
 | fin_delay: forall st st' tr, fin tr st' -> fin (Tcons st tr) st'.
 
 Lemma append_fin: forall (p q : trace -> Prop) tr0 tr1, p tr0 -> q tr1 -> fin tr0 (hd tr1) ->
-(p *+* q) (tr0 +++ tr1).
+  (p *+* q) (tr0 +++ tr1).
 Proof.
 move => p q tr0 tr1 hp hq hfin. exists tr0. split => // {hp}.
 move: tr0 tr1 hq hfin. cofix CIH. case=> st0 tr0.
 - move => hq h1. rewrite trace_append_nil. inv h1. by apply: follows_nil.
 - move => tr1 h0 h1. inv h1. rewrite [Tcons st0 tr0 +++ tr1]trace_destr /=.
-  by apply/follows_delay/(CIH _ _ h0).
+  by apply/follows_delay/CIH.
 Qed.
 
 Definition last (p: trace -> Prop): assertS :=
-fun st => exists tr, (p tr) /\ (fin tr st).
+  fun st => exists tr, p tr /\ fin tr st.
 
 Lemma last_cont: forall (p q: trace -> Prop),
-(forall tr, p tr -> q tr) ->
-last p ->> last q.
+  (forall tr, p tr -> q tr) ->
+  last p ->> last q.
 Proof.
 move => p0 p1 hp st [tr [h0 h1]].
 exists tr. split=>//. by apply: hp.
 Qed.
 
 Definition Last (p: assertT): assertS.
-move: p => [f0 h0]. by apply (last f0).
+move: p => [f0 h0]. by apply: last.
 Defined.
 
 (* Proposition 3.2: Last is monotone. *)
 Lemma Last_monotone: forall p q,
-p =>> q -> Last p ->> Last q.
+  p =>> q -> Last p ->> Last q.
 Proof.
 move=> [f hf] [g hg] /= h0.
 by apply/last_cont/h0.
@@ -903,7 +887,7 @@ Qed.
 Lemma Last_Singleton_unfold: forall u, u ->> Last ([|u|]).
 Proof.
 move => u st0 h0. exists (Tnil st0). split.
-- exists st0. by split=>//; apply: bisim_nil.
+- by exact: mk_singleton_nil.
 - by apply: fin_nil.
 Qed.
 
@@ -914,79 +898,75 @@ Proof.
 move => p q st [tr0] [[tr [_ h2]] h1].
 move: tr0 st h1 tr h2. induction 1=> tr0 h0; inv h0.
 - exists (Tnil st). by split=>//; apply: fin_nil.
-- exists (Tcons st tr). by split=>//; apply: (fin_delay _ h1).
-- by apply: (IHh1 _ H1).
+- exists (Tcons st tr). by split=>//; apply: fin_delay.
+- by apply/IHh1/H1.
 Qed.
 
 (* Lemma 3.4, (13) *)
 Lemma Last_chop_sglt: forall p v,
-Last (p *** [|v|]) ->> v.
+  Last (p *** [|v|]) ->> v.
 Proof.
 move => [p hp] v /= st [tr [[tr' [_ h0]] h1]].
 move: tr st h1 tr' h0. induction 1=> tr0 h0; inv h0.
 - move: H0 => [st0 [h0 h1]]. by inv h1.
 - move: H0 => [st0 [_ h0]]. by inv h0.
-- by apply: (IHh1 _ H1).
+- by apply/IHh1/H1.
 Qed.
 
 Lemma Last_andS: forall p u, ((Last p) andS u) ->> Last (p *** [|u|]).
 Proof.
-move => [p hp] u st0 [/= [tr0 [h2 h3]] h1].
+move => [p hp] u st0 [/= [tr0][h2 h3] h1].
 exists tr0. split=>//. exists tr0. split=>// {h2}.
 move: tr0 st0 h3 h1. cofix CIH=> tr0 st0 h0. inv h0=> h0.
-- apply follows_nil => //. exists st0. by split=>//; apply: bisim_reflexive.
-- by apply/follows_delay/(CIH _ _ H).
+- by apply/follows_nil/mk_singleton_nil.
+- by apply/follows_delay/CIH/h0.
 Qed.
 
 Lemma iter_last: forall v,
-([|v|] *** (Iter (ttT *** Dup v))) =>> (ttT *** [|v|]).
+  ([|v|] *** (Iter (ttT *** Dup v))) =>> (ttT *** [|v|]).
 Proof.
-move => v tr0 [tr1 [[st0 [h0 h2]] h1]]. inv h2.
-inv h1. simpl. exists tr0. split => //. move: tr0 h0 H1.
-cofix CIH=> tr0 h0 h1. inv h1.
-- apply follows_nil => //. simpl in h0. exists st.
-  by split=>//; apply: bisim_nil.
-- clear h0. move: H => [tr1 [_ h1]]. move: tr1 tr tr0 h1 H0.
+move => v tr0 [tr1][[st0][h0 h2] h1]. inv h2. inv h1=>/=.
+exists tr0. split => //.
+move: tr0 h0 H1. cofix CIH=> tr0 h0 h1. inv h1.
+- by apply/follows_nil/mk_singleton_nil.
+- move: H => {h0} [tr1 [_ h1]]. move: tr1 tr tr0 h1 H0.
   cofix CIH0=> tr0 tr1 tr2 h0 h1. inv h0.
   - move: H0 => [st0 [h0 h2]]. inv h2. inv H1. inv h1. inv H2.
-    by apply/follows_delay/(CIH _ h0).
-  - inv h1. by apply/follows_delay/(CIH0 _ _ _ H).
+    by apply/follows_delay/CIH.
+  - inv h1. by apply/follows_delay/CIH0/H3/H.
 Qed.
 
 (* Lemma 3.4, (14) *)
 Lemma Last_Sglt_Iter: forall v p,
-Last ([|v|] *** (Iter (p *** Dup v))) ->> v.
+  Last ([|v|] *** (Iter (p *** Dup v))) ->> v.
 Proof.
 move => v p st0 h0.
-have h1: p =>> ttT by done.
-have {}h0 := Last_monotone (Append_monotone_R (Iter_monotone (Append_monotone_L
-h1))) h0 => {h1}.
-move: (Last_monotone (@iter_last v) h0) => {h0}.
-by apply: Last_chop_sglt.
+apply: (@Last_chop_sglt ttT).
+apply/Last_monotone/Last_monotone/h0; first by apply: iter_last.
+by apply/Append_monotone_R/Iter_monotone/Append_monotone_L.
 Qed.
 
 Lemma iter_last_dup: forall v,
-(<<v>> *** (Iter (ttT *** <<v>>))) =>> (ttT *** [|v|]).
+  (<<v>> *** (Iter (ttT *** <<v>>))) =>> (ttT *** [|v|]).
 Proof.
 move=> v tr0 [tr1 [[st0 [h0 h2]] h1]].
 inv h2. inv H1. inv h1. inv H2. simpl.
 exists (Tcons (hd tr') tr'). split => //.
-apply follows_delay => //. move: tr' h0 H1.
-cofix CIH=> tr0 h0 h1. inv h1.
-- apply follows_nil => //. simpl in h0. exists st.
-  by split => //; apply: bisim_nil.
-- clear h0. move: H => [tr1 [_ h1]]. move: tr1 tr tr0 h1 H0.
-  cofix CIH0=> tr0 tr1 tr2 h0 h1. inv h0.
+apply follows_delay => //.
+move: tr' h0 H1. cofix CIH=> tr0 h0 h1. inv h1.
+- by apply/follows_nil/mk_singleton_nil.
+- move: H => {h0} [tr1 [_ h1]].
+  move: tr1 tr tr0 h1 H0. cofix CIH0=> tr0 tr1 tr2 h0 h1. inv h0.
   - move: H0 => [st0 [h0 h2]]. inv h2. inv H1. inv h1. inv H2.
-    by apply/follows_delay/(CIH _ h0).
-  - inv h1. by apply/follows_delay/(CIH0 _ _ _ H).
+    by apply/follows_delay/CIH.
+  - inv h1. by apply/follows_delay/CIH0/H3/H.
 Qed.
 
 (* Lemma 3.4, (12) *)
 Lemma Last_Last: forall p q,
-(Last ([| Last p |] *** q)) ->> (Last (p *** q)).
+  (Last ([| Last p |] *** q)) ->> (Last (p *** q)).
 Proof.
-move => [p hp] [q hq] st0 /= [tr1 [[tr0 [[tr2 [h0 h3]] h2]] h1]].
+move => [p hp] [q hq] st0 /= [tr1][[tr0][[tr2][h0 h3] h2] h1].
 inv h3. inv h2. move: h0 => [tr2 [h0 h2]].
 exists (tr2 +++ tr1). split.
 * exists tr2. split => // {h0 h1}.
@@ -1003,12 +983,12 @@ exists (tr2 +++ tr1). split.
 Qed.
 
 Lemma singleton_andS_append: forall u v,
-(v andS u) ->> Last ([|v|] *** [|u|]).
+  (v andS u) ->> Last ([|v|] *** [|u|]).
 Proof.
 move => u v st0 [h0 h1]. exists (Tnil st0). split.
 * exists (Tnil st0). split.
-  - exists st0. by split => //; apply bisim_reflexive.
-  - apply: follows_nil=>//. exists st0. by split => //; apply: bisim_reflexive.
+  - by exact: mk_singleton_nil.
+  - by apply/follows_nil/mk_singleton_nil.
 * by apply: fin_nil.
 Qed.
 
@@ -1027,12 +1007,12 @@ exists (lastdup tr0). split.
   have h4 := follows_setoid (@singleton_setoid _) h2 h3 (bisim_reflexive _) => {h2}.
   exists tr0. split.
   - by apply: (hp _ h0 _ h3).
-  - by apply: (follows_dup h4).
-* by apply: (fin_lastdup h1).
+  - by apply: follows_dup.
+* by apply: fin_lastdup.
 Qed.
 
-Lemma hd_append: forall tr0 st0, fin tr0 st0 -> forall tr1,
-hd tr1 = st0 -> hd (tr0 +++ tr1) = hd tr0.
+Lemma hd_append: forall tr0 st0, fin tr0 st0 ->
+  forall tr1, hd tr1 = st0 -> hd (tr0 +++ tr1) = hd tr0.
 Proof.
 induction 1=> tr0 h0.
 - by rewrite trace_append_nil.
