theories/SemaxComplete.v
@@ -11,13 +11,11 @@ Lemma conv_follows: forall (u:assertS) tr,
 Proof.
 move => u. cofix CIH. case=> st0.
 - move => h0.
-  have h1 := h0 st0 (fin_nil st0) => {h0}.
-  apply follows_nil=>//. exists st0.
-  by split=>//; apply: bisim_reflexive.
+  apply/follows_nil/mk_singleton_nil=>//.
+  by apply/h0/fin_nil.
 - move => tr0 h0.
-  have h1: forall st, fin tr0 st -> u st.
-  * move => st1 h1. by apply: (h0 st1 (fin_delay st0 h1)).
-  by apply: (follows_delay st0 (CIH _ h1)).
+  apply/follows_delay/CIH=>st1 h1.
+  by apply/h0/fin_delay.
 Qed.
 
 Lemma last_adequate: forall (p: trace -> Prop) tr, p tr ->
@@ -40,7 +38,7 @@ Inductive loopinv (a: expr) (sp: assertS -> trace -> Prop) (u:assertS) : assertS
   loopinv a sp u st
 | loopinv_next: forall st tr st' (v: assertS),
   loopinv a sp u st ->
-  is_true (a st) = true ->
+  is_true (a st) ->
   hd tr = st ->
   (forall st, v st -> loopinv a sp u st) ->
   sp v tr ->
@@ -49,14 +47,14 @@ Inductive loopinv (a: expr) (sp: assertS -> trace -> Prop) (u:assertS) : assertS
 
 Fixpoint sp (s: stmt) (u: assertS) {struct s} : trace -> Prop :=
 match s with
-| Sskip => (singleton u)
-| Sassign x a => (updt u x a)
+| Sskip => singleton u
+| Sassign x a => updt u x a
 | Sseq s1 s2 =>
    append (sp s1 u) (sp s2 (last (sp s1 u)))
 | Sifthenelse a s1 s2 =>
   append (dup u)
   (fun tr => sp s1 (u andS eval_true a) tr \/ sp s2 (u andS eval_false a) tr)
-|Swhile a s =>
+| Swhile a s =>
   let I := loopinv a (sp s) u in
   append (dup u)
   (append
@@ -73,23 +71,22 @@ Qed.
 Lemma sp_hd: forall s u tr, sp s u tr -> u (hd tr).
 Proof.
 move => s; induction s => /= u tr.
-- move => [st [h1 h2]]. subst. inv h2. simpl. by apply h1.
-- move => [st0 [h1 h2]]. inv h2. inv H1. simpl. by apply h1.
+- move => [st [h1 h2]]. by inv h2.
+- move => [st0 [h1 h2]]. inv h2. by inv H1.
 - move => [tr0 [h1 h2]].
-  have h3 := IHs1 _ _ h1.
-  rewrite (follows_hd h2) in h3; by apply h3.
+  move: (IHs1 _ _ h1); by rewrite (follows_hd h2).
 - move => [tr0 [[st1 [h1 h3]] h2]]. inv h3. inv H1. by inv h2.
 - move => [tr0 [[st1 [h1 h3]] h2]]. inv h3. inv H1. by inv h2.
 Qed.
 
 Lemma loopinv_cont: forall e (sp: assertS -> trace -> Prop),
-(forall u u', u ->> u' -> forall tr, sp u tr -> sp u' tr) ->
-forall u u',  u ->> u' -> loopinv e sp u ->> loopinv e sp u'.
+  (forall u u', u ->> u' -> forall tr, sp u tr -> sp u' tr) ->
+  forall u u',  u ->> u' -> loopinv e sp u ->> loopinv e sp u'.
 Proof.
 move => e sp0 hsp0. rewrite /assertS_imp in hsp0 *.
-move => u u' h1 . induction 1.
+move => u u' h1. induction 1.
 - by apply/loopinv_here/h1.
-- by apply: loopinv_next; [exact: IHloopinv| |exact: H1|exact: H3 | | ].
+- by apply/(loopinv_next IHloopinv)/H5/H4.
 Qed.
 
 (* Lemma 3.7: sp is monotone. *)
@@ -97,10 +94,8 @@ Lemma sp_cont: forall s u u',
  u ->> u' -> forall tr, sp s u tr -> sp s u' tr.
 Proof.
 move => s; induction s => /= u0 u1 h1 tr0 h2 /=.
-- move: h2 => [st1 [h2 h3]]. inv h3. exists st1.
-  by split; [apply: (h1 _ h2)| apply: bisim_reflexive].
-- move: h2 => [st0 [h3 h2]]. inv h2. inv H1. exists st0.
-  by split; [apply: (h1 _ h3)| apply: bisim_reflexive].
+- move: h2 => [st1 [h2 h3]]. inv h3. by apply/mk_singleton_nil/h1.
+- move: h2 => [st0 [h3 h2]]. inv h2. inv H1. by apply/mk_updt/h1.
 - move: h2 => [tr1 [h3 h4]]. exists tr1. split.
   * by apply: (IHs1 _ _ h1 _ h3).
   * clear h3. move: tr1 tr0 h4. cofix CIH=> tr0 tr1 h2.
@@ -109,29 +104,25 @@ move => s; induction s => /= u0 u1 h1 tr0 h2 /=.
       apply: IHs2 _ _ _ _ H0. by apply/last_cont/(IHs1 _ _ h1).
     - by apply/follows_delay/CIH/H.
 - move: h2 => [tr1 [[st0 [h2 h4]] h3]].
-  inv h4. inv h3. inv H1. inv H3. exists (Tcons (hd tr') (Tnil (hd tr'))). split.
-  * exists (hd tr'). by split; [apply: (h1 _ h2) | apply: bisim_reflexive].
-  * apply/follows_delay/follows_nil=>//.
-    move: H1 => [h6 | h6].
-    - left. apply: IHs1 h6 => st0 [h6 h7].
-      split=>//; by apply: h1 h6.
-    - right. apply: IHs2 h6 => st0 [h6 h7].
-      split=>//; by apply: h1 h6.
+  inv h4. inv h3. inv H1. inv H3.
+  exists (Tcons (hd tr') (Tnil (hd tr'))). split; first by apply/mk_dup/h1.
+  apply/follows_delay/follows_nil=>//.
+  case: H1 => h6.
+  - left. apply: IHs1 h6 => st0 [h6 h7].
+    split=>//; by apply: h1 h6.
+  - right. apply: IHs2 h6 => st0 [h6 h7].
+    split=>//; by apply: h1 h6.
 - move: h2 => [tr1 [[st0 [h2 h4]] h3]].
   inv h4. inv h3. inv H1. inv H3.
-  exists (Tcons (hd tr') (Tnil (hd tr'))). split.
-  * exists (hd tr'). by split; [apply: (h1 _ h2) | apply: bisim_reflexive].
-  * apply/follows_delay/follows_nil=>//.
-    have h3 := loopinv_cont IHs h1.
-    have h4 := h3 e => {h3}.
-    have h5 := dup_cont h4.
-    have h3: (loopinv e (sp s) u0 andS eval_true e) ->>
-      (loopinv e (sp s) u1 andS eval_true e)
-      by move => st0 [h0 h3]; split => //; apply: (h4 _ h0).
-    have h6 := IHs _ _ h3 => {h4 h3}.
-    have h3 := append_cont h6 h5 => {h6 h5}.
-    have h4 := iter_cont h3 => {h3}.
-    by apply: (append_cont_L h4 H1).
+  exists (Tcons (hd tr') (Tnil (hd tr'))). split; first by apply/mk_dup/h1.
+  apply/follows_delay/follows_nil=>//.
+  have h3 := loopinv_cont IHs h1.
+  have h4 := h3 e => {h3}.
+  have h3: (loopinv e (sp s) u0 andS eval_true e) ->>
+           (loopinv e (sp s) u1 andS eval_true e)
+    by move => st0 [h0 h3]; split => //; apply: h4.
+  apply/append_cont_L/H1/iter_cont/append_cont; last by apply: dup_cont h4.
+  by apply: IHs.
 Qed.
 
 (* Lemma 3.11: any trace satisfying sp(s,U) is produced by a run of s. *)
@@ -140,37 +131,34 @@ sp s u  tr ->
 exec s (hd tr) tr.
 Proof.
 move => s; induction s =>/=.
-- move => u tr [st [h1 h2]]. inv h2. simpl. by apply: exec_skip.
-- move => u tr [st [h1 h2]]. inv h2. inv H1. simpl. apply: exec_assign.
+- move => u tr [st [h1 h2]]. inv h2=>/=. by apply: exec_skip.
+- move => u tr [st [h1 h2]]. inv h2. inv H1=>/=. apply: exec_assign.
 - move => u tr [tr0 [h1 h2]].
   have h3:= IHs1 _ _ h1.
   have h4 := follows_hd h2.
   rewrite h4 in h3.
   apply: (exec_seq h3) => {h1 h4 h3}.
   move: tr0 tr h2. cofix CIH=> tr0 tr1 h1. inv h1.
-  - by apply/execseq_nil/(IHs2 _ _ H0).
-  - by apply/execseq_cons/(CIH _  _ H).
+  - by apply/execseq_nil/IHs2/H0.
+  - by apply/execseq_cons/CIH.
 - move => u tr [tr0 [[st0 [h1 h3]] h2]].
-  inv h3. inv h2. inv H1. inv H3. simpl. case: H1 => h4.
+  inv h3. inv h2. inv H1. inv H3=>/=. case: H1 => h4.
   - move: (sp_hd h4) => [h5 h6].
     apply: (exec_ifthenelse_true _ h6).
-    apply: execseq_cons. apply: execseq_nil.
-    by apply: (IHs1 _ _ h4).
+    by apply/execseq_cons/execseq_nil/IHs1/h4.
   - move: (sp_hd h4) => [h5 h6].
     apply: (exec_ifthenelse_false _ h6).
-    apply: execseq_cons. apply: execseq_nil.
-    by apply: (IHs2 _ _ h4).
+    by apply/execseq_cons/execseq_nil/IHs2/h4.
 - move => u tr0 [tr1 [[st0 [h1 h3]] h2]].
-  inv h3. inv H1. inv h2. inv H2. simpl. move => {h1}.
+  inv h3. inv H1. inv h2. inv H2=>/= {h1}.
   move: H1 => [tr0 [h0 h1]]. move: tr' tr0 h0 h1. cofix CIH.
   have h: forall tr2 tr tr1 tr0: trace, follows (dup (loopinv e (sp s) u)) tr2 tr ->
-  follows
-  (iter (append (sp s (loopinv e (sp s) u andS eval_true e))
-          (dup (loopinv e (sp s) u)))) tr tr1 ->
-  follows (singleton (eval_false e)) tr1 tr0 -> execseq (Swhile e s) tr2 tr0.
+    follows (iter (append (sp s (loopinv e (sp s) u andS eval_true e))
+                  (dup (loopinv e (sp s) u)))) tr tr1 ->
+    follows (singleton (eval_false e)) tr1 tr0 -> execseq (Swhile e s) tr2 tr0.
   * cofix CIH0=> tr0 tr1 tr2 tr3 h0 h2 h3.
     inv h0. move: H0 => [st0 [_ h1]].
-    inv h1. inv H1. inv h2. inv H2. inv h3. simpl.
+    inv h1. inv H1. inv h2. inv H2. inv h3=>/=.
     rewrite (follows_hd H3).
     apply/execseq_nil/(CIH _ _ H1 H3).
     inv h2. inv h3.
@@ -190,27 +178,25 @@ Qed.
 
 (* Lemma 3.6: sp is setoid. *)
 Lemma sp_setoid: forall s u tr tr',
-sp s u tr -> bisim tr tr' -> sp s u tr'.
+  sp s u tr -> bisim tr tr' -> sp s u tr'.
 Proof.
 move => s; induction s => /= u tr0 tr1.
 - move => [st0 [h1 h2]] h3. inv h2. inv h3.
-  exists st0. by split=>//; apply: bisim_reflexive.
+  by exact: mk_singleton_nil.
 - move => [st0 [h1 h2]] h3. inv h2. inv H1. inv h3. inv H2.
-  exists st0. by split=>//; apply: bisim_reflexive.
+  by exact: mk_updt.
 - move => [tr2 [h1 h2]] h3. exists tr2. split.
   * apply: (IHs1 _ _ _ h1). by apply: bisim_reflexive.
-  * move => {h1}. move: tr0 tr1 tr2 h3 h2.
-    cofix CIH=> tr0 tr1 tr2 h3 h2. inv h2.
+  * move => {h1}. move: tr0 tr1 tr2 h3 h2. cofix CIH=> tr0 tr1 tr2 h3 h2. inv h2.
     - apply: follows_nil; first by apply/esym/(bisim_hd h3).
       by apply: (IHs2 _ _ _ H0).
     - inv h3. by apply: (follows_delay st (CIH _ _ _ H3 H)).
 - move => [tr2 [[st0 [h1 h4]] h2]] h3. inv h4.
   inv H1. inv h2. inv h3. inv H2.
   have h2 := bisim_hd H3.
-  exists (Tcons (hd tr') (Tnil (hd tr'))). split.
-  * exists (hd tr'). by split; [apply h1 | reflexivity].
+  exists (Tcons (hd tr') (Tnil (hd tr'))). split; first by exact: mk_dup.
   apply/follows_delay/follows_nil; first by apply/esym.
-  clear h1 h2. move: H1 => [h1 | h1].
+  clear h1 h2. case: H1 => h1.
   - left. apply: (IHs1 _ _ _ h1 H3).
   - right. apply: (IHs2 _ _ _ h1 H3).
 - move => [tr2 [h0 h2]] h1. exists tr2.
@@ -222,27 +208,26 @@ Qed.
 
 (* Lemma 3.9: => *)
 Lemma loopinv_adequate: forall a s u tr,
-sp s (loopinv a (sp s) u andS eval_true a) tr ->
-append (sp s (loopinv a (sp s) u andS eval_true a))
-             (singleton (loopinv a (sp s) u)) tr.
+  sp s (loopinv a (sp s) u andS eval_true a) tr ->
+  append (sp s (loopinv a (sp s) u andS eval_true a))
+               (singleton (loopinv a (sp s) u)) tr.
 Proof.
 move => a s u tr h0. exists tr. split=>//.
 apply: conv_follows => st0 h1.
-move: (sp_hd h0) => [h2 h3]. inv h3.
-have h3 := @andS_left (loopinv a (sp s) u) (eval_true a).
-have h4 := sp_cont h3 h0 => {h3 h0}.
-by apply: (loopinv_next h2 H0 _ _ h4).
+move: (sp_hd h0) => [h2 h3]. rewrite /is_true in h3.
+have h4 := @andS_left (loopinv a (sp s) u) (eval_true a).
+have h5 := sp_cont h4 h0 => {h4 h0}.
+by apply: (loopinv_next h2 h3 _ _ h5).
 Qed.
 
 (* Lemma 3.9: <= *)
 Lemma loopinv_adequate_aux: forall a s u tr,
-append (sp s (loopinv a (sp s) u andS eval_true a))
-             (singleton (loopinv a (sp s) u)) tr ->
-sp s (loopinv a (sp s) u andS eval_true a) tr.
+  append (sp s (loopinv a (sp s) u andS eval_true a))
+               (singleton (loopinv a (sp s) u)) tr ->
+  sp s (loopinv a (sp s) u andS eval_true a) tr.
 Proof.
 move => a s u tr0 [tr1 [h0 h1]].
-move: (follows_singleton h1) => {}h1.
-by apply: (sp_setoid h0 h1).
+by apply/sp_setoid/follows_singleton/h1.
 Qed.
 
 Definition Sp (s: stmt) (u: assertS): assertT.
@@ -254,14 +239,12 @@ Defined.
 Lemma sp_deducible: forall s u, semax u s (Sp s u).
 Proof.
 move => s; induction s => u.
-- have h0: ([|u|]) =>> (Sp Sskip u).
-  * move => tr0 [st0 [h0 h1]]. inv h1. exists st0.
-    by split; [apply h0 | reflexivity].
-  by apply: (semax_conseq_R h0 (semax_skip _)).
-- have h0: (Updt u i e) =>> Sp (i <- e) u.
-  * move => tr0 h0. move: h0 => [st0 [h0 h1]]. inv h1. inv H1.
-     exists st0. by split=>//; apply: bisim_reflexive.
-  by apply: (semax_conseq_R h0 (semax_assign _ _ _)).
+- apply/semax_conseq_R/semax_skip.
+  move => tr0 [st0 [h0 h1]]. inv h1=>/=.
+  by exact: mk_singleton_nil.
+- apply/semax_conseq_R/semax_assign.
+  move => tr0 [st0 [h0 h1]]. inv h1. inv H1=>/=.
+  by exact: mk_updt.
 - have h0 := IHs1 u => {IHs1}.
   have h1 := (@Last_adequate (Sp s1 u)).
   have h2 := semax_conseq_R h1 h0 => {h0 h1}.
@@ -297,13 +280,11 @@ Qed.
 
 (* Corollary 3.2 *)
 Lemma sp_correct: forall s (u: assertS) (p: assertT),
-(forall st tr, exec s st tr -> u st -> satisfy p tr) ->
-forall tr, sp s u tr -> satisfy p tr.
+  (forall st tr, exec s st tr -> u st -> satisfy p tr) ->
+  forall tr, sp s u tr -> satisfy p tr.
 Proof.
 move => s u p h1 tr h2.
-have h3 := sp_then_exec h2.
-have h4 := sp_hd h2.
-apply: (h1 _ _ h3 h4).
+apply/h1/(sp_hd h2)/sp_then_exec/h2.
 Qed.
 
 (* Proposition 3.4: Completeness *)
