theories/Hoare.v
@@ -5,7 +5,7 @@ Unset Strict Implicit.
 Import Prenex Implicits.
 
 Definition udt (u: assertS) (x: id) (a: expr): assertS :=
-fun st => exists st0 : state, (u st0) /\ (update x (a st0) st0 = st).
+  fun st => exists st0 : state, (u st0) /\ (update x (a st0) st0 = st).
 
 Inductive hsemax : assertS -> stmt -> assertS -> Prop :=
 
@@ -39,17 +39,15 @@ Inductive hsemax : assertS -> stmt -> assertS -> Prop :=
   hsemax (exS u) s (exS v).
 
 Lemma hsemax_conseq_L: forall s u1 u2 v,
-u1 ->> u2 -> hsemax u2 s v -> hsemax u1 s v.
+  u1 ->> u2 -> hsemax u2 s v -> hsemax u1 s v.
 Proof.
-move => s u1 u2 v h0 h1.
-by exact: hsemax_conseq h0 (@assertS_imp_refl v) h1.
+move => s u1 u2 v h0 h1. by apply/hsemax_conseq/h1.
 Qed.
 
 Lemma hsemax_conseq_R: forall s u v1 v2,
 v2 ->> v1 -> hsemax u s v2 -> hsemax u s v1.
 Proof.
-move => s u v1 v2 h0 h1.
-by apply: (hsemax_conseq (@assertS_imp_refl u) h0 h1).
+move => s u v1 v2 h0 h1. by apply/hsemax_conseq/h1.
 Qed.
 
 Lemma Last_destruct : forall (p: assertT) st tr,
@@ -64,19 +62,16 @@ Lemma semax_correct_hsemax: forall u s p,
 semax u s p -> forall v, hsemax (v andS u) s (Last ([|v|] *** p)).
 Proof.
 induction 1.
-- move => v. have h0 := hsemax_skip (v andS u).
-  have h1 := (@singleton_andS_append u v).
-  by apply: (hsemax_conseq_R h1 h0).
-- move => v. have h0 := hsemax_assign (v andS u) x a.
-  have h1: (udt (v andS u) x a) ->> (Last ([|v|] *** Updt u x a)).
-  * move => st0 [st1 [[{}h0 h1] h2]].
-    exists (Tcons st1 (Tnil st0)). split.
-    + exists (Tnil st1). split.
-      - exists st1; split => //. by apply bisim_reflexive.
-      apply: follows_nil=>//. rewrite /updt. exists st1. split => //.
-      rewrite h2. by apply: bisim_reflexive.
-    by apply/fin_delay/fin_nil.
-  by apply: (hsemax_conseq_R h1 h0).
+- move => v.
+  by apply/hsemax_conseq_R/hsemax_skip/singleton_andS_append.
+- move => v.
+  apply/hsemax_conseq_R/hsemax_assign.
+  move => st0 [st1 [[{}h0 h1] h2]].
+  exists (Tcons st1 (Tnil st0)). split.
+  + exists (Tnil st1). split; first by exact: mk_singleton_nil.
+    rewrite -h2.
+    by apply/follows_nil/mk_updt.
+  by apply/fin_delay/fin_nil.
 - move => v0.
   have h: Last ([|Last ([|v0|] *** p1 *** [|v|])|] *** p2) ->>
   Last ([|v0|] *** p1 *** p2).
@@ -93,26 +88,18 @@ induction 1.
   have hpost : (Last ([|v andS u|] *** p)) ->> (Last ([|v|] *** <<u>> *** p)).
   * destruct p as [p hp]. move => st0 [tr0 [[tr1 [[st1 [h4 h3]] h2]] h1]] /=.
      inv h3. inv h2. move: h4 => [h2 h3]. exists (Tcons (hd tr0) tr0).
-     split.
-     + exists (Tnil (hd tr0)). split.
-       - exists (hd tr0). split => //. by apply bisim_reflexive.
-       apply follows_nil =>//.
-       exists (Tcons (hd tr0) (Tnil (hd tr0))). split.
-       - exists (hd tr0). split => //. by apply bisim_reflexive.
-       apply/follows_delay/follows_nil =>//. by apply: fin_delay.
+     split; last by apply: fin_delay.
+     exists (Tnil (hd tr0)). split; first by exact: mk_singleton_nil.
+     apply follows_nil =>//.
+     exists (Tcons (hd tr0) (Tnil (hd tr0))). split; first by exact: mk_dup.
+     by apply/follows_delay/follows_nil.
   apply hsemax_ifthenelse.
-  * have hpre: ((v andS u) andS eval_true a) ->>
-     ((v andS u) andS u andS eval_true a).
-      * move => st0 [h0 h1]. split => //. move: h0 => [h0 h2]. by split.
-     have h0 := IHsemax1 (v andS u) => {IHsemax1}.
-     move: (hsemax_conseq_L hpre h0) => {}h0.
-     apply: (hsemax_conseq_R hpost h0).
-  * have hpre: ((v andS u) andS eval_false a) ->>
-     ((v andS u) andS u andS eval_false a).
-      * move => st0 [h0 h1]. split => //. move: h0 => [h0 h2]. by split.
-     have h0 := IHsemax2 (v andS u) => {IHsemax1 IHsemax2}.
-     move: (hsemax_conseq_L hpre h0) => {}h0.
-     apply: (hsemax_conseq_R hpost h0).
+  * apply/hsemax_conseq_R/hsemax_conseq_L/(IHsemax1 (v andS u))=>//.
+    (* hpre *)
+    by move => st0 [[h0 h2] h1].
+  * apply/hsemax_conseq_R/hsemax_conseq_L/(IHsemax2 (v andS u))=>//.
+    (* hpre *)
+    by move => st0 [[h0 h2] h1].
 - move => w.
   set inv := Last ([|w|] *** <<u0>> *** Iter ( p *** <<u>>)).
   have h0 := IHsemax inv => {IHsemax H0}.
@@ -124,10 +111,8 @@ induction 1.
     inv H2. inv h2. inv h1. inv H3.
     have h0 := H _ h3 => {h3}.
     have h1: satisfy (ttT *** [|u|]) tr'.
-    * apply: iter_last=>/=. exists (Tnil (hd tr')). split.
-      - exists (hd tr'). by split => //; apply: bisim_nil.
-      apply follows_nil => //.
-      by apply: (iter_cont (@append_cont_L _ _ _ _) H2).
+    * apply: iter_last=>/=. exists (Tnil (hd tr')). split; first by exact: mk_singleton_nil.
+      by apply/follows_nil/iter_cont/H2/append_cont_L.
     simpl in h1. clear H2 h0. move: h1 => [tr0 [_ h1]].
     move: tr' st H4 tr0 h1. induction 1 => tr0 h0; inv h0.
     - move: H1 => [st0 [h0 h1]]. by inv h1.
@@ -151,22 +136,21 @@ induction 1.
   apply: (hsemax_conseq _ _ h0).
   * move => st0 {}h0. rewrite /inv.
     apply: (Last_monotone
-    (@Append_monotone_R _ _ _ (@Append_monotone_R  _ _ _ (@Stop_Iter _)))).
-    move: h0 => [h0 h1]. exists (Tcons st0 (Tnil st0)). split.
-    + exists (Tnil st0). split.
-      - exists st0. split => //. by apply: bisim_reflexive.
-      apply: follows_nil=>//. exists (Tcons st0 (Tnil st0)). split.
-      - exists st0. split => //. by apply bisim_reflexive.
-      apply/follows_delay/follows_nil=>//. exists st0. split => //. by apply bisim_reflexive.
-    by apply/fin_delay/fin_nil.
+             (@Append_monotone_R _ _ _ (@Append_monotone_R  _ _ _ (@Stop_Iter _)))).
+    move: h0 => [h0 h1].
+    exists (Tcons st0 (Tnil st0)). split; last by apply/fin_delay/fin_nil.
+    exists (Tnil st0). split; first by apply: mk_singleton_nil.
+    apply: follows_nil=>//.
+    exists (Tcons st0 (Tnil st0)). split; first by exact: mk_dup.
+    by apply/follows_delay/follows_nil/mk_singleton_nil.
   * rewrite /inv => st0 [h1 h2].
     apply: (Last_monotone (@Append_assoc_L _ _ _)).
     apply: (Last_monotone (@Append_assoc_L _ _ _)).
     apply: (Last_monotone (@Append_monotone_L _ _ _ (@Append_assoc_R _ _ _))).
     destruct p as [p hp]. move: h1 => [tr0 [h1 h3]] /=.
-    exists tr0. split => //. exists tr0. split => // {h1}. move: tr0 h3.
-    cofix CIH=> tr0 h1. inv h1.
-    + apply follows_nil=>//. exists st0. split => //. by apply: bisim_reflexive.
+    exists tr0. split => //. exists tr0. split => // {h1}.
+    move: tr0 h3. cofix CIH=> tr0 h1. inv h1.
+    - by apply/follows_nil/mk_singleton_nil.
     by apply/follows_delay/CIH.
 - move => v.
   have h := IHsemax v => {IHsemax}.
@@ -176,14 +160,14 @@ induction 1.
   by apply/Last_monotone/Append_monotone_R.
 - move => v.
   have h0: (v andS exS u) ->> (exS (fun a => v andS u a)).
-  * move => st0 [h0 [x h1]]. exists x. by split.
+  * move => st0 [h0 [x h1]]. by exists x.
   apply: (hsemax_conseq_L h0) => {h0}.
   have h0: (exS (fun x => Last ([|v|] *** (p x)))) ->> Last ([|v|] *** exT p).
   * move => st0 [x h0]. move hp: (p x) => [q hq].
     rewrite hp /= in h0. destruct h0 as [tr0 [h0 h1]].
     exists tr0. split => // {h1}. destruct h0 as [tr1 [h0 h1]].
-    exists tr1. split => // {h0}. move: tr1 tr0 h1.
-    cofix CIH=> tr0 tr1 h0. inv h0.
+    exists tr1. split => // {h0}.
+    move: tr1 tr0 h1. cofix CIH=> tr0 tr1 h0. inv h0.
     - apply follows_nil => //. exists x. by rewrite hp.
     by apply/follows_delay/CIH.
   apply: (hsemax_conseq_R h0)=>{h0}.
@@ -192,77 +176,57 @@ Qed.
 
 (* Corollary 4.2 *)
 Lemma semax_correct_hsemax_main: forall u s p,
-semax u s p -> hsemax u s (Last p).
+  semax u s p -> hsemax u s (Last p).
 Proof.
 move => U s P hhsemax.
 move: (semax_correct_hsemax hhsemax ttS) => {}hhsemax.
-apply: (hsemax_conseq _ _ hhsemax) => {hhsemax}st0.
- * move => hU. by split.
- * move => h0. destruct P as [P hP]. destruct h0 as [tr0 [h0 h1]].
-   exists tr0. split => //. destruct h0 as [h0 [h2 h3]].
-   inv h2. destruct H as [_ h2]. clear h1.
-   inv h2. inversion h3; by subst.
+apply: (hsemax_conseq _ _ hhsemax) => // {hhsemax}st0 h0.
+destruct P as [P hP]. destruct h0 as [tr0 [h0 h1]].
+exists tr0. split => //. destruct h0 as [h0 [h2 h3]].
+inv h2. destruct H as [_ h2]. clear h1.
+inv h2. inversion h3; by subst.
 Qed.
 
 (* Proposition 4.1: embedding the partial-correctness Hoare logic
    into the trace-based Hoare logic *)
 Lemma hsemax_correct_semax: forall u s v,
-hsemax u s v -> semax u s (ttT *** [|v|]).
+  hsemax u s v -> semax u s (ttT *** [|v|]).
 Proof.
 induction 1.
-- have h0 := semax_skip u.
-  have h1: ([|u|]) =>> (ttT *** [|u|]).
-  * move => tr0 [st0 [h1 h2]]. inv h2. exists (Tnil st0). split => //.
-    apply follows_nil =>//. exists st0. by split=>//; apply: bisim_nil.
-  by apply: (semax_conseq_R h1 h0).
-- have h0 := semax_assign u x a.
-  have h1: (Updt u x a) =>> (ttT *** [|udt u x a|]).
-  * move => tr0 [st0 [h1 h2]]. exists tr0. split => //. inv h2. inv H1.
-    apply/follows_delay/follows_nil=>//.
-    exists (update x (a st0) st0).
-    split; last by apply bisim_nil. exists st0. by split.
-  by apply: (semax_conseq_R h1 h0).
+- apply/semax_conseq_R/semax_skip.
+  move => tr0 [st0 [h1 h2]]. inv h2. exists (Tnil st0). split => //.
+  by apply/follows_nil/mk_singleton_nil.
+- apply/semax_conseq_R/semax_assign.
+  move => tr0 [st0 [h1 h2]]. exists tr0. split => //. inv h2. inv H1.
+  apply/follows_delay/follows_nil=>//.
+  exists (update x (a st0) st0). split; last by apply bisim_nil. by exists st0.
 - have h0 := semax_seq IHhsemax1 IHhsemax2 => {IHhsemax1 IHhsemax2}.
   have h1 := semax_conseq_R (@Append_assoc_R _ _ _) h0 => {h0}.
   apply: (semax_conseq_R (@Append_monotone_L _ _ _ (@ttT_idem_comp)) h1).
-- have h0 := semax_ifthenelse IHhsemax1 IHhsemax2 => {IHhsemax1 IHhsemax2 H H0}.
-  have h1: (<<u1>> *** ttT *** [|u2|]) =>> (ttT *** [|u2|]).
-  * move => tr0 {}h0. move: (append_assoc_R h0) => [tr1 [{}h0 h1]].
-    exists tr1. by split.
-  by apply: (semax_conseq_R h1 h0).
-- have h0: u ->> u by [].
-  have h1 := semax_while h0 IHhsemax => {h0 IHhsemax}.
-  set p0 := (ttT *** << u >>).
-  have h0: ((<< u >>) *** Iter p0 *** [|eval_false a|]) =>>
-  (ttT *** [|u andS eval_false a|]).
-  * move => tr0 [tr1 [[st0 [h0 h2]] {}h1]].
-    inv h2. inv H2. inv h1. inv H3. exists (Tcons (hd tr') tr').
-    split=>//. apply follows_delay. move: tr' H2 h0.
-    cofix CIH0=> tr0 [tr1 [h0 h2]] h1.
-    inv h0.
-    + inv h2. move: H2 => [st0 [h0 h2]]. inv h2. simpl in h1.
-      apply follows_nil => //. exists st0. split => //. by apply: bisim_reflexive.
-    clear h1. move: tr tr1 tr0 H0 H1 h2.
-    cofix CIH1=> tr0 tr1 tr2 [tr3 [h0 h3]] h1 h2. inv h3.
-    + clear h0. move: H1 => [st0 [h0 h3]]. inv h3. inv H2. inv h1.
-      inv H3. inv h2. rewrite (follows_hd H4) in h0.
-      apply: (follows_delay (hd tr')); apply: (CIH0 _ _ h0).
-      by exists tr'.
-    inv h1. inv h2.
-    clear h0 CIH0. apply follows_delay.
-    apply: (CIH1 _ _ _ _ H4 H5). by exists tr.
-  by apply: (semax_conseq_R h0 h1).
-- have h0 := Singleton_monotone H0.
-  have h1 := (@Append_monotone_R ttT _ _ h0) => {h0}.
-  have h0 := semax_conseq_R h1 IHhsemax => {h1 IHhsemax}.
-  apply: (semax_conseq_L H h0).
-- have h0: (exT (fun x => ttT *** [|v x|])) =>> (ttT *** [|exS v|]).
-  * move => tr0 [x /= [tr1 [h0 h1]]].
-    exists tr1. split => // {h0}. move: tr1 tr0 h1.
-    cofix CIH=> tr0 tr1 h0. inv h0.
-    + apply follows_nil => //. destruct H2 as [st0 [h0 h1]].
-      exists st0; split => //. by exists x.
-    by apply/follows_delay/CIH.
-  apply: (semax_conseq_R h0) => {h0}.
-  by apply semax_ex.
+- apply/semax_conseq_R/(semax_ifthenelse IHhsemax1 IHhsemax2) => {IHhsemax1 IHhsemax2 H H0}.
+  move => tr0 h0. move: (append_assoc_R h0) => [tr1 [{}h0 h1]].
+  by exists tr1.
+- apply/semax_conseq_R/semax_while/IHhsemax=>//.
+  move => tr0 [tr1 [[st0 [h0 h2]] h1]].
+  inv h2. inv H2. inv h1. inv H3.
+  exists (Tcons (hd tr') tr'). split=>//. apply follows_delay.
+  move: tr' H2 h0. cofix CIH0=> tr0 [tr1 [h0 h2]] h1. inv h0.
+  + inv h2. move: H2 => [st0 [h0 h2]]. inv h2. simpl in h1.
+    by apply/follows_nil/mk_singleton_nil.
+  clear h1.
+  move: tr tr1 tr0 H0 H1 h2. cofix CIH1=> tr0 tr1 tr2 [tr3 [h0 h3]] h1 h2. inv h3.
+  + clear h0. move: H1 => [st0 [h0 h3]].
+    inv h3. inv H2. inv h1. inv H3. inv h2. rewrite (follows_hd H4) in h0.
+    apply/follows_delay/(CIH0 _ _ h0). by exists tr'.
+  inv h1. inv h2.
+  clear h0 CIH0.
+  apply/follows_delay/(CIH1 _ _ _ _ H4 H5). by exists tr.
+- by apply/semax_conseq_L/semax_conseq_R/IHhsemax/Append_monotone_R/Singleton_monotone.
+- apply/semax_conseq_R/semax_ex/H0.
+  move => tr0 [x /= [tr1 [h0 h1]]].
+  exists tr1. split => // {h0}.
+  move: tr1 tr0 h1. cofix CIH=> tr0 tr1 h0. inv h0.
+  + apply follows_nil => //. destruct H2 as [st0 [h0 h1]].
+    exists st0; split => //. by exists x.
+  by apply/follows_delay/CIH.
 Qed.
