theories/HoareTotal.v
@@ -1,13 +1,14 @@
-From CoindSemWhile Require Import SsrExport Trace Language Semax SemaxSound.
-From CoindSemWhile Require Import Assert AssertClassical BigFunct.
+From CoindSemWhile Require Import SsrExport Trace Language BigFunct.
+From CoindSemWhile Require Import Assert AssertClassical Semax SemaxSound.
 From Coq Require Import Lia Program.Equality.
 
 Set Implicit Arguments.
 Unset Strict Implicit.
 Import Prenex Implicits.
 
+(* copied from Hoare *)
 Definition udt (u: assertS) (x: id) (a: expr): assertS :=
-fun st => exists st0 : state, (u st0) /\ ((update x (a st0) st0) = st).
+  fun st => exists st0 : state, (u st0) /\ (update x (a st0) st0 = st).
 
 Inductive tsemax2: assertS -> stmt -> assertS -> Prop :=
 
@@ -42,43 +43,33 @@ Inductive tsemax2: assertS -> stmt -> assertS -> Prop :=
   tsemax2 (exS u) s (exS v).
 
 Lemma tsemax2_conseq_L: forall s u1 u2 v,
-u1 ->> u2 -> tsemax2 u2 s v -> tsemax2 u1 s v.
+  u1 ->> u2 -> tsemax2 u2 s v -> tsemax2 u1 s v.
 Proof.
 move => s u1 u2 v h0 h1.
-by apply: (tsemax2_conseq h0 _ h1).
+by apply/tsemax2_conseq/h1.
 Qed.
 
 Lemma tsemax2_conseq_R: forall s u v1 v2,
 v2 ->> v1 -> tsemax2 u s v2 -> tsemax2 u s v1.
 Proof.
 move => s u v1 v2 h0 h1.
-by apply: (tsemax2_conseq _ h0 h1).
+by apply/tsemax2_conseq/h1.
 Qed.
 
 Lemma tsemax2_false: forall s u, tsemax2 ffS s u.
 Proof.
 move => s. induction s=>u.
-- have hs := tsemax2_skip ffS.
-  by apply: (tsemax2_conseq_R _ hs).
-- have hs := tsemax2_assign ffS.
-  by apply: (tsemax2_conseq_R _ (hs _ _)) => {hs} st0 [st1 [h0 _]].
-- have hs1 := IHs1 ffS => {IHs1}.
-  have hs2 := IHs2 u => {IHs2}.
-  by apply: (tsemax2_seq hs1 hs2).
-- have hs1 := IHs1 u => {IHs1}.
-  have hs2 := IHs2 u => {IHs2}.
-  have htrue : (ffS andS eval_true e) ->> ffS
-    by move => st0 [h0 h1].
-  have hfalse : (ffS andS eval_false e) ->> ffS
-    by move => st0 [h0 h1].
-  by exact: (tsemax2_ifthenelse (tsemax2_conseq_L htrue hs1) (tsemax2_conseq_L hfalse hs2)).
+- by apply/tsemax2_conseq_R/tsemax2_skip.
+- by apply/tsemax2_conseq_R/tsemax2_assign=>st0 [st1][h0 _].
+- by apply/tsemax2_seq/IHs2.
+- by apply/tsemax2_ifthenelse;
+    (apply/tsemax2_conseq_L; first by exact: andS_left).
 - set J := fun m: nat => ffS.
-  have hs: forall n, tsemax2 (eval_true e andS J n) s (exS (fun k => (fun st => k < n)
-  andS (J k))).
-  * move => n.
-    apply: (tsemax2_conseq _ _ (IHs (exS (fun k => (fun st => k < n) andS J k))))=> //.
-    by rewrite /J => st [_ h].
-  by apply: (tsemax2_conseq _ _ (tsemax2_while 0 hs)) =>// st0 [n0 [h0 [h1 h2]]].
+  apply/tsemax2_conseq/(tsemax2_while 0 (J:=J))=>//.
+  - by move=>st0 [n0][h0 [h1 _]].
+  move => n.
+  apply: (tsemax2_conseq _ _ (IHs (exS (fun k => (fun st => k < n) andS J k))))=>//.
+  by rewrite /J => st [_ h].
 Qed.
 
 Inductive len: nat -> trace -> Prop :=
@@ -91,7 +82,7 @@ by induction 1; [apply: len_stop|apply: len_delay].
 Qed.
 
 Lemma len_monotone: forall n m, n <= m ->
-forall tr, len n tr -> len m tr.
+  forall tr, len n tr -> len m tr.
 Proof.
 move=> n m h0 tr h1.
 rewrite (_: m = (m - n) + n); last by lia.
@@ -103,10 +94,10 @@ move=> {n m tr h0 h1}p. induction p=>q tr.
 Qed.
 
 Definition Len (p: assertT) (n: nat) : assertS :=
-fun st => forall tr, (hd tr = st) /\ (satisfy p tr) -> len n tr.
+  fun st => forall tr, (hd tr = st) /\ (satisfy p tr) -> len n tr.
 
 (* Lemma 4.1: ⌈P⌉n is anti-monotone. *)
-Lemma Len_monotone: forall n p q, q =>> p -> (Len p n) ->> (Len q n).
+Lemma Len_monotone: forall n p q, q =>> p -> Len p n ->> Len q n.
 Proof.
 move => n p q hpq st0. rewrite /Len => hp tr0 [h0 h1].
 apply hp. split => //. by apply: hpq.
@@ -115,17 +106,16 @@ Qed.
 Lemma Len_monotone2: forall p n m, n <= m -> Len p n ->> Len p m.
 Proof.
 move => p n m hnm st0 h0 tr0 [h1 h2].
-have {h1 h2}h0 : len n tr0 by apply h0.
-by apply: (len_monotone hnm).
+by apply/(len_monotone hnm)/h0.
 Qed.
 
 Definition after (p: assertT) (q: assertT) :=
-let: exist p hp := p in let: exist q hq := q in
-forall tr, p tr -> exists tr0: trace, follows q tr tr0.
+  let: exist p hp := p in let: exist q hq := q in
+  forall tr, p tr -> exists tr0: trace, follows q tr tr0.
 
 (* Lemma 4.2: ◃ is monotone on the left argument . *)
 Lemma after_monotone_L: forall p0 p1 q, p0 =>> p1 ->
-after p1 q -> after p0 q.
+  after p1 q -> after p0 q.
 Proof.
 move => [p0 hp0] [p1 hp1] [q hq] h0 h1 tr1 h2.
 move: (h0 _ h2) => /= {}h2.
@@ -183,7 +173,7 @@ move => u0 w u p st0 a0 h2.
 have {h2}h4 : Last ((<< u >>) *** Iter (ttT *** (<< u >>))) st0.
 * apply/(Last_monotone _ h2)/Append_monotone.
   - move => tr0 [st1 [h4 h5]] /=. inv h5. inv H1. destruct h4 as [h4 h5].
-    exists st1. by split; [apply: a0|apply: bisim_reflexive].
+    by apply/mk_dup/a0.
   - by apply/Iter_monotone/Append_monotone_L.
 by apply: (Last_chop_sglt (Last_monotone (@iter_last_dup _) h4)).
 Qed.
@@ -195,10 +185,10 @@ move => [p hp] [q hq] [r hr] /= h0 tr0 [tr1 [[st0 [h1 h3]] h2]].
 inv h3. inv h2. destruct h1 as [tr1 [h1 h2]].
 have h3: (p *+* q) (tr1 +++ tr0).
 * exists tr1; split => // {h1}. move: tr0 tr1 H1 h2.
-  cofix hcoind=> tr0. case=>st0.
+  cofix CIH=> tr0. case=>st0.
   - move=>h2 h1. inv h1. rewrite trace_append_nil. by apply follows_nil.
   - move=>tr1 h2 h3. inv h3. rewrite [Tcons st0 tr1 +++ _]trace_destr /=.
-    by apply/follows_delay/(hcoind _ _ h2).
+    by apply/follows_delay/(CIH _ _ h2).
 move: (h0 _ h3) => {h0 H1 h1 h3}[tr2 h0].
 move h1 : (hd tr0) => st0. rewrite h1 in h2. move: tr1 st0 h2 tr0 h1 tr2 h0.
 induction 1=> tr0 h0 tr1 h1.
@@ -212,8 +202,7 @@ Qed.
 Lemma after_Last: forall p r, after ([|Last p|]) r -> after p r.
 Proof.
 move => [p hp] [q hq] /= h0 tr0 h1.
-apply: fin_hd_follows.
-exact: (singleton_last_fin h0).
+by apply/fin_hd_follows/singleton_last_fin/h1.
 Qed.
 
 (* Proposition 4.4: projecting the total-correctness Hoare logic into
@@ -227,30 +216,23 @@ induction 1.
   have h0 := tsemax2_skip (u andS w andS Len (([|u|]) *** r) m).
   apply: (tsemax2_conseq_R _ h0) => st [{}h0 [h1 h2]].
   split.
-  * exists (Tnil st). split.
-    + exists (Tnil st). split.
-      - exists st. by split => //; apply: bisim_reflexive.
-      apply follows_nil => //.
-      exists st. by split => //; apply: bisim_reflexive.
-    apply fin_nil.
+  * exists (Tnil st). split; last by exact: fin_nil.
+    exists (Tnil st). split; first by exact: mk_singleton_nil.
+    by apply/follows_nil/mk_singleton_nil.
   move => tr [h3 h4]. apply h2. split => //. destruct r as [r hr]. simpl.
-  simpl in h4. exists (Tnil st). split.
-  * exists st. by split => //; apply: bisim_reflexive.
-  by apply: follows_nil.
+  simpl in h4. exists (Tnil st).
+  by split; [exact: mk_singleton_nil| exact: follows_nil].
 - move => m w r hafter.
   have h0 := tsemax2_assign (u andS w andS Len (Updt u x a *** r) m) x a.
   apply: (tsemax2_conseq_R _ h0) => st [st1 [[{}h0 [h2 h3]] h1]].
   split.
-  * exists (Tcons st1 (Tnil st)). split.
-    + exists (Tnil st1). split.
-      - exists st1. by split => //; apply: bisim_reflexive.
-      apply follows_nil => //. exists st1. split => //. rewrite h1. by apply: bisim_reflexive.
-    by apply/fin_delay/fin_nil.
+  * exists (Tcons st1 (Tnil st)). split; last by apply/fin_delay/fin_nil.
+    exists (Tnil st1). split; first by exact: mk_singleton_nil.
+    rewrite -h1. by apply/follows_nil/mk_updt.
   move => tr0 [h4 h5].
   have {h1 h2 h3 h4 h5}h0: len m (Tcons st1 tr0).
   * apply h3 => {h3}. split => //. destruct r as [r hr]. simpl. exists (Tcons st1 (Tnil st)).
-    split.
-    + exists st1. split => //. rewrite h1. by apply: bisim_reflexive.
+    split; first by rewrite -h1; exact: mk_updt.
     by apply/follows_delay/follows_nil.
   inv h0. by apply: len_S.
 - move => m w r hafter.
@@ -274,7 +256,8 @@ induction 1.
   have hs1 := IHsemax1 m w (p2 *** r) hr => {IHsemax1 hr}.
   have h0: (Len ((p1 *** p2) *** r) m) ->> Len ((p1 *** [|v|]) *** p2 *** r) m.
   * apply Len_monotone. apply: (impT_conseq_L (@Append_monotone_L _ p1 _ _)).
-    apply Append_Singleton. by apply Append_assoc_R.
+    - by apply: Append_Singleton.
+    by apply Append_assoc_R.
   have {h0}hs1 : tsemax2 (u andS w andS Len ((p1 *** p2) *** r) m)
                s1 (Last (([|w|]) *** p1 *** ([|v|])) andS Len (p2 *** r) m).
   * apply: (tsemax2_conseq_L _ hs1) => {hs1} st0 [h1 [h2 h3]].
@@ -319,11 +302,9 @@ induction 1.
       simpl in hafter. move => tr0 [tr1 [h0 h1]]. destruct h0 as [st0 [h0 h2]].
       inv h2. inv h1. destruct h0 as [h0 h1].
       have h2: (singleton w *+* dup u *+* p) (Tcons (hd tr0) tr0).
-      * exists (Tnil (hd tr0)). split.
-        + exists (hd tr0). by split => //; apply: bisim_reflexive.
+      * exists (Tnil (hd tr0)). split; first by exact: mk_singleton_nil.
         apply follows_nil => //. exists (Tcons (hd tr0) (Tnil (hd tr0))).
-        split.
-        + exists (hd tr0). by split => //; apply: bisim_reflexive.
+        split; first by exact: mk_dup.
         by apply/follows_delay/follows_nil.
       move: (hafter _ h2) => {h0 h1 h2} [tr1 h3]. inv h3.
       by exists tr'.
@@ -334,44 +315,36 @@ induction 1.
         move: (Len_monotone (@Append_assoc_R _ _ _) h3) => {}h3.
         destruct p as [p hp]. destruct r as [r hr]. move => tr0 [{}h1 /= {}h2].
         have f4 : ((dup u) *+* (p *+* r)) (Tcons (hd tr0) tr0).
-        + exists (Tcons (hd tr0) (Tnil (hd tr0))). split.
-          - exists (hd tr0). by split; [rewrite h1|apply/bisim_reflexive].
+        + exists (Tcons (hd tr0) (Tnil (hd tr0))). split; first by rewrite h1; exact: mk_dup.
           by apply/follows_delay/follows_nil.
         have h5: len m (Tcons (hd tr0) tr0) by apply: h3.
         inv h5. by exact: len_S H3.
        * move => st0 [h0 h1]. split => // {h1}. destruct p as [p hp].
          destruct h0 as [tr0 [h0 h1]]. exists (Tcons (hd tr0) tr0).
          destruct h0 as [tr1 [h0 h2]]. destruct h0 as [st1 [h0 h3]].
-         inv h3. inv h2. destruct h0 as [h0 h2]. split.
-         + exists (Tnil (hd tr0)). split.
-           - exists (hd tr0). by split => //; apply: bisim_reflexive.
-           apply follows_nil => //.
-           exists (Tcons (hd tr0) (Tnil (hd tr0))). split.
-           - exists (hd tr0). by split => //; apply: bisim_reflexive.
-           by apply/follows_delay/follows_nil.
-      by apply: fin_delay.
+         inv h3. inv h2. destruct h0 as [h0 h2]. split; last by exact: fin_delay.
+         exists (Tnil (hd tr0)). split; first by exact: mk_singleton_nil.
+         apply follows_nil => //.
+         exists (Tcons (hd tr0) (Tnil (hd tr0))). split; first by exact: mk_dup.
+         by apply/follows_delay/follows_nil.
     move: (IHsemax2 m _ _ haftertt) => {IHsemax2 haftertt} hsemax.
     apply: (tsemax2_conseq _ _ hsemax) => {hsemax}.
     * move => st0 [[h0 [h1 h3]] h2]. split => //. split => //.
       move: (Len_monotone (@Append_assoc_R _ _ _) h3) => {}h3.
       destruct p as [p hp]. destruct r as [r hr]. move => tr0 [{}h1 /= {}h2].
       have h4 : ((dup u) *+* (p *+* r)) (Tcons (hd tr0) tr0).
-      + exists (Tcons (hd tr0) (Tnil (hd tr0))). split.
-        - exists (hd tr0); by split; [rewrite h1|apply: bisim_reflexive].
+      + exists (Tcons (hd tr0) (Tnil (hd tr0))). split; first by rewrite h1; exact: mk_dup.
         by apply/follows_delay/follows_nil.
       have h5: len m (Tcons (hd tr0) tr0) by apply: h3.
       inv h5. by exact: len_S H3.
      * move => st0 [h0 h1]. split => //. clear h1. destruct p as [p hp].
        destruct h0 as [tr0 [h0 h1]]. exists (Tcons (hd tr0) tr0).
        destruct h0 as [tr1 [h0 h2]]. destruct h0 as [st1 [h0 h3]].
-       inv h3. inv h2. destruct h0 as [h0 h2]. split.
-       + exists (Tnil (hd tr0)). split.
-         - exists (hd tr0). by split => //; apply: bisim_reflexive.
-         apply follows_nil => //.
-         exists (Tcons (hd tr0) (Tnil (hd tr0))). split.
-         - exists (hd tr0). by split => //; apply: bisim_reflexive.
-         by apply/follows_delay/follows_nil.
-       by apply: fin_delay.
+       inv h3. inv h2. destruct h0 as [h0 h2]. split; last by exact: fin_delay.
+       exists (Tnil (hd tr0)). split; first by exact: mk_singleton_nil.
+       apply follows_nil => //.
+       exists (Tcons (hd tr0) (Tnil (hd tr0))). split; first by exact: mk_dup.
+       by apply/follows_delay/follows_nil.
 - move => m w r hafter.
   set J0 := Last (<< u0 andS w >> *** (Iter (p *** << u >>))).
   set J1 := (Iter (p *** << u >>) *** [|eval_false a|] *** r).
@@ -383,7 +356,7 @@ induction 1.
   have hn0: (eval_true a andS J0 andS Len J1 0) ->> ffS.
   * move => st0. rewrite /J0 /J1. move => [h1 [h2 h3]].
     have hfalse: forall tr0, satisfy (Iter (p *** <<u>>) *** [|eval_false a|] *** r) tr0
-    -> hd tr0 = st0 -> False.
+      -> hd tr0 = st0 -> False.
     * destruct p as [p hp]. destruct r as [r hr]. simpl. move => tr0 h4 h5.
        have {}h3 : len 0 tr0 by apply h3.
        destruct h4 as [tr1 [h4 h6]]. inv h4.
@@ -404,7 +377,7 @@ induction 1.
                    *** [|eval_false a|]) r.
      * apply: (after_monotone_L _ hafter) => {hafter}.
        apply/Append_monotone_R/Append_monotone_R.
-       apply: (assertT_imp_trans (@Append_assoc_R _ _ _)).
+       apply: (impT_conseq_L (@Append_assoc_R _ _ _)).
        by apply/Append_monotone_L/Iter_Iter.
 
     set P := ([|w|] *** << u0 >> *** Iter (p *** <<u>>) *** Iter (p *** <<u>>) *** [|eval_false a|]).
@@ -417,20 +390,18 @@ induction 1.
     have h5 : append (iter (append p (dup u)))
              (append (iter (append p (dup u))) (singleton (eval_false a))) (tr' +++ tr'0).
     * exists tr'. split => // {hu hfalse H2 h2 h0 h4 h1 h3}. move: tr' tr'0 H4 H3.
-      cofix hcoind=> tr0 tr1 h0. inv h0=>h0.
+      cofix CIH=> tr0 tr1 h0. inv h0=>h0.
       - apply follows_nil => //. by rewrite trace_append_nil.
       rewrite [Tcons st tr +++ tr1]trace_destr/=.
-      apply follows_delay. by exact: (hcoind _ _ H0 h0).
+      by apply/follows_delay/CIH/h0.
     have hP : satisfy P (Tcons (hd tr') (tr' +++ tr'0)).
-    * rewrite /P /=. exists (Tnil (hd tr')). split.
-      - exists (hd tr'). by split => //; apply: bisim_reflexive.
+    * rewrite /P /=. exists (Tnil (hd tr')). split; first by exact: mk_singleton_nil.
       apply follows_nil => //.
-      exists (Tcons (hd tr') (Tnil (hd tr'))). split.
-      - exists (hd tr'). by split => //; apply bisim_reflexive.
+      exists (Tcons (hd tr') (Tnil (hd tr'))). split; first by exact: mk_dup.
       apply/follows_delay/follows_nil => //. by apply: (hd_append H4 (refl_equal _)).
     simpl in hfalse. rewrite -trace_append_cons in hP.
     have hfinite: fin (Tcons (hd tr') tr') (hd tr'0) by apply fin_delay.
-    clear H4. clear h3.
+    clear H4 h3.
     move: (hafter _ hP) => {hP hafter} [tr0 h3].
     move heq: (Tcons (hd tr') tr') => tr1.
     rewrite heq in h3 hfinite.
@@ -443,7 +414,7 @@ induction 1.
   (* end of hn0 *)
 
   have hpre: forall n, (eval_true a andS J0 andS Len J1 n) ->>
-  (eval_true a andS u andS J0 andS Len (p *** [|u|] *** Q) n).
+    (eval_true a andS u andS J0 andS Len (p *** [|u|] *** Q) n).
   * move => n st0 [h0 [h1 h2]]. split => //. split => //.
     + rewrite /J0 in h1.
       have h3:((<< u0 andS w >>) *** Iter (p *** (<< u >>)))
@@ -451,7 +422,7 @@ induction 1.
       - apply Append_monotone.
         + apply: Dup_monotone => st1 [h3 h4]. by exact: (H _ h3).
         by apply/Iter_monotone/Append_monotone_L.
-      have {}h3 := assertT_imp_trans h3 (@iter_last_dup _).
+      have {}h3 := impT_conseq_L h3 (@iter_last_dup _).
       have {}h3 := Last_monotone h3.
       move: (h3 _ h1) => {h3 h1}.
       by apply: Last_chop_sglt.
@@ -489,8 +460,7 @@ induction 1.
       have h4 : len n (Tcons (hd tr0) tr0).
       + apply: h1=>/=. split => //.
         have hu := tsemax2_complete_aux3 H h0.
-        exists (Tcons (hd tr0) (Tnil (hd tr0))). split.
-        - exists (hd tr0). by split => //; [rewrite h2 | apply: bisim_reflexive].
+        exists (Tcons (hd tr0) (Tnil (hd tr0))). split; first by rewrite h2; exact: mk_dup.
         by apply/follows_delay/follows_nil.
       inv h4. by rewrite (_: S n0 - 1 = n0); last by lia.
     fold J0 in h0. fold J1 in h0. exists (n-1). destruct h0 as [h0 h1].
@@ -513,147 +483,151 @@ induction 1.
     * move => st0 [h0 [h1 [h2 h3]]]. split => //. split => // tr0 [h4 h5].
       apply h3. split => //.
       move: (@Append_assoc_L _ _ _ _ h5) => {}h5.
-      destruct p as [p hp]. destruct r as [r hr].
-      simpl. simpl in h5. exists (Tnil (hd tr0)). split.
-      - exists st0. by split => //; rewrite h4; apply: bisim_reflexive.
-    by apply: follows_nil.
+      destruct p as [p hp]. destruct r as [r hr]. simpl. simpl in h5.
+      exists (Tnil (hd tr0)). split; first by rewrite h4; apply: mk_singleton_nil.
+      by apply: follows_nil.
 
 (* prove after ([J0] *** p *** [u]) Q *)
     rewrite /J0. apply after_Append.
     move: (after_monotone_L (@Append_assoc_L _ _ _) hafter) => {}hafter.
     have h0: <<u0 andS w>> =>> [|w|] *** <<u0>>.
     * move => tr0 /= [st0 [h0 h1]]. inv h1. inv H3. destruct h0 as [h0 h1].
-      exists (Tnil st0). split.
-      - exists st0. by split => //; apply: bisim_reflexive.
-      apply follows_nil => //. exists st0. by split => //; apply: bisim_reflexive.
+      exists (Tnil st0). split; first by exact: mk_singleton_nil.
+      by apply/follows_nil/mk_dup.
     move: (after_monotone_L (Append_monotone_L h0) hafter) => {h0}hafter.
 
     have h0: after (<< u0 andS w >> *** Iter (p *** << u >>) *** p *** [|u|])
     (<< u >> *** Iter (p *** << u >>) *** [|eval_false a|]).
-    * have := after_monotone_L (@Append_assoc_R _ _ _). apply.
-      have := after_monotone_L (@Append_assoc_R _ _ _). apply.
+    * apply: (after_monotone_L (@Append_assoc_R _ _ _)).
+      apply: (after_monotone_L (@Append_assoc_R _ _ _)).
       apply after_Last.
-      have := after_monotone_L (Singleton_monotone (@Last_chop_sglt _ _)).
-      apply. clear hafter.
+      apply: (after_monotone_L (Singleton_monotone (@Last_chop_sglt _ _))) => {hafter}.
       have hsemax := semax_while (@assertS_imp_refl _) H0 => {H0}.
       have h0 := semax_total hsemax => {hsemax}.
-      destruct p as [p hp]. simpl. move => tr0 [st0 [h1 h2]]. inv h2.
-      have := h0 _ h1 => {h0 h1}. move => [tr0 [h0 h1]]. simpl in h1.
+      destruct p as [p hp]. move => /= tr0 [st0 [h1 h2]]. inv h2.
+      move: (h0 _ h1) => [tr0 [{}h0 /= {}h1]].
       exists tr0. apply follows_nil => //.
 
   (** end of h0 **)
 
-   destruct p as [p hp]. rewrite /Q. destruct r as [r hr]. simpl.
-   simpl in hafter. simpl in h0. move => tr0 h1.
+   destruct p as [p hp]. rewrite /Q. destruct r as [r hr].
+   simpl. simpl in hafter. simpl in h0. move => tr0 h1.
    move: (append_assoc_L h1) => {}h1.
-   have := h0 _ h1 => {h0}. move => [tr1 h0].
-   have :((dup (u0 andS w) *+* iter (p *+* dup u) *+* p *+* singleton u)
-   *+* (dup u *+* iter (p *+* dup u) *+* singleton (eval_false a))) tr1.
-   exists tr0. split => //. clear h1. move => h3.
+   move: (h0 _ h1) => [tr1 {}h0].
+   have h3 : ((dup (u0 andS w) *+* iter (p *+* dup u) *+* p *+* singleton u)
+     *+* (dup u *+* iter (p *+* dup u) *+* singleton (eval_false a))) tr1.
+     by exists tr0.
    have: (dup (u0 andS w) *+* iter (p *+* dup u) *+* singleton (eval_false a)) tr1.
-   * clear h0. have := append_assoc_L h3. move => h0.
-     have := append_monotone_R _ h0. apply. clear h0. move => tr2 h0.
-     have := append_assoc_R h0 => {h0}. move => h0.
-     have := append_assoc_R h0 => {h0}. move => h0.
-     have := append_cont_L _ h0 => {h0}. apply. clear tr2.
-     move => tr2 h0. have := append_assoc_L h0 => {h0}. move => h0.
-     have := append_assoc_L h0 => {h0}. move => h0.
-     have : forall tr, ((p *+* singleton u) *+* dup u *+* iter (p *+* dup u)) tr ->
+   * move: (append_assoc_L h3) => {}h0.
+     apply: (append_monotone_R _ h0) => tr2 {}h0.
+     move: (append_assoc_R h0) => {}h0.
+     move: (append_assoc_R h0) => {}h0.
+     apply: (append_cont_L _ h0) => {}tr2 {}h0.
+     move: (append_assoc_L h0) => {}h0.
+     move: (append_assoc_L h0) => {}h0.
+     have {}h1 : forall tr, ((p *+* singleton u) *+* dup u *+* iter (p *+* dup u)) tr ->
      iter (p *+* dup u) tr.
-     * clear tr0 h0. move => tr0 h0. have := append_assoc_R h0 => {h0}.
-       move => [tr3 [h0 h1]]. have := iter_loop _ h1. apply. clear h1.
-       have := append_cont_L _ h0. apply. apply append_singleton => //.
-     move => h1. have := append_monotone_R h1 h0 => {h0 h1}. move => h0.
-     have := iter_iter h0. done.
-   clear h3. move => h1. have := hafter _ h1 => {h1}. move => [tr2 h1].
-   exists tr2. have := follows_monotone (@append_assoc_L _ _ _). apply.
-   have := follows_monotone (@append_assoc_L _ _ _). apply.
-   have := follows_follows h0 h1 => {h0 h1}. clear tr1. move => h0.
-   have := follows_monotone (append_cont_L (@append_assoc_R _ _ _)) h0 => {h0}. done.
+     * move => {h1}tr0 {}h0.
+       move: (append_assoc_R h0) => [tr3 [{}h0 h1]].
+       apply: (iter_loop _ h1) => {h1}.
+       apply: (append_cont_L _ h0).
+       by apply: append_singleton.
+     move: (append_monotone_R h1 h0) => {h1}h0.
+     by exact: iter_iter h0.
+   move => {h3}h1.
+   move: (hafter _ h1) => [tr2 {}h1].
+   exists tr2.
+   apply: (follows_monotone (@append_assoc_L _ _ _)).
+   apply: (follows_monotone (@append_assoc_L _ _ _)).
+   move: (follows_follows h0 h1) => {h1 tr1}h0.
+   by apply: (follows_monotone (append_cont_L (@append_assoc_R _ _ _)) h0).
 
-  have := (@tsemax2_while _ _ m _ hs). clear hs. move => hs.
+  move: (@tsemax2_while _ _ m _ hs) => {}hs.
   have hpre: (u0 andS w andS Len ((<<u0>> *** Iter (p *** <<u>>) ***
-  [| eval_false a|]) *** r) m) ->> J0 andS Len J1 m.
+    [| eval_false a|]) *** r) m) ->> J0 andS Len J1 m.
   * have h0: (u0 andS w) ->> J0.
-     * move => st0 [h0 h1]. rewrite /J0. destruct p as [p hp]. simpl.
-        exists (Tcons st0 (Tnil st0)). split. exists (Tcons st0 (Tnil st0)). split.
-        exists st0. split => //. apply bisim_reflexive. apply follows_delay.
-        apply follows_nil => //. apply iter_stop. apply fin_delay. apply fin_nil.
-     have h1: (u0 andS Len ((<<u0>> *** Iter (p *** <<u>>) *** [|eval_false a|]) *** r) m) ->>
-     Len J1 m.
-     * destruct p as [p hp]. destruct r as [r hr]. move => st0. move => [h1 h2].
-        rewrite /J1. move => tr0 [h4 h3]. simpl in h3.
-        have h5: len m (Tcons (hd tr0) tr0).
-        * apply h2. simpl. split => //. destruct h3 as [tr1 [h3 h5]].
-           have h6 := follows_hd h5. exists (Tcons (hd tr1) tr1). split.
-           exists (Tcons (hd tr1) (Tnil (hd tr1))).  split. exists (hd tr1). split => //.
-           rewrite h6. rewrite h4. done. apply bisim_reflexive. apply follows_delay.
-           apply follows_nil => //. exists tr1. split => //.
-           clear h0 h1 h2 h4 h3 h6. move: tr1 tr0 h5. cofix hcoind.
-           move => tr0 tr1 h0. inv h0. destruct H2 as [tr0 [h0 h1]].
-           destruct h0 as [st1 [h0 h2]]. inv h2. inv h1. apply follows_nil => //.
-           exists (hd tr1). split => //. apply bisim_reflexive. apply follows_delay.
-           have := hcoind _ _ H1. done.
-           rewrite h6. apply follows_delay. clear h0 h1 h2 h3 h4 h6. move: tr1 tr0 h5.
-           cofix hcoind. move => tr0 tr1 h0. inv h0. destruct H2 as [tr0 [h0 h1]].
-           destruct h0 as [st1 [h0 h2]]. inv h2. inv h1. apply follows_nil => //.
-           apply follows_delay. have := hcoind _ _ H1. done.
-        inv h5. have := len_S H3. done.
-        move => st0 [h2 [h3 h4]]. split. apply h0. split => //. apply h1.
-        split => //.
-  have := tsemax2_conseq_L hpre. apply. clear hpre.
+    * move => st0 [h0 h1]. rewrite /J0. destruct p as [p hp]. simpl.
+      exists (Tcons st0 (Tnil st0)). split; last by apply/fin_delay/fin_nil.
+      exists (Tcons st0 (Tnil st0)). split; first by apply: mk_dup.
+      by apply/follows_delay/follows_nil/iter_stop.
+    have h1: (u0 andS Len ((<<u0>> *** Iter (p *** <<u>>) *** [|eval_false a|]) *** r) m) ->>
+      Len J1 m.
+    * destruct p as [p hp]. destruct r as [r hr]. move => st0 [h1 h2].
+      rewrite /J1. move => tr0 [h4 h3]. simpl in h3.
+      have h5: len m (Tcons (hd tr0) tr0).
+      * apply h2=>/=. split => //. destruct h3 as [tr1 [h3 h5]].
+        have h6 := follows_hd h5. exists (Tcons (hd tr1) tr1). split.
+        - exists (Tcons (hd tr1) (Tnil (hd tr1))). split; first by rewrite h6 h4; exact: mk_dup.
+          apply/follows_delay/follows_nil => //.
+          exists tr1. split => //. clear h0 h1 h2 h4 h3 h6.
+          move: tr1 tr0 h5. cofix CIH=> tr0 tr1 h0. inv h0.
+          - destruct H2 as [tr0 [h0 h1]]. destruct h0 as [st1 [h0 h2]]. inv h2. inv h1.
+            by apply/follows_nil/mk_singleton_nil.
+          by apply/follows_delay/CIH/H1.
+        rewrite h6. apply follows_delay. clear h0 h1 h2 h3 h4 h6.
+        move: tr1 tr0 h5. cofix CIH=>tr0 tr1 h0. inv h0.
+        - destruct H2 as [tr0 [h0 h1]]. destruct h0 as [st1 [h0 h2]]. inv h2. inv h1.
+          by exact: follows_nil.
+        by apply/follows_delay/CIH/H1.
+      inv h5. by exact: len_S H3.
+    move => st0 [h2 [h3 h4]]. by split; [apply: h0|apply: h1].
+  apply: (tsemax2_conseq_L hpre) => {hpre}.
   have hpost : (exS (fun k => (fun _ => k <= m) andS
-  (J0 andS Len J1 k) andS eval_false a)) ->> J0 andS Len J1 m andS eval_false a.
-  * move => st0 [x h0]. destruct h0 as [h0 [[h1 h2] h3]].
-    split => //. split => //. have := Len_monotone2 h0 h2. done.
-  have := tsemax2_conseq_R hpost hs. clear hpost hs. move => hs.
+    (J0 andS Len J1 k) andS eval_false a)) ->> J0 andS Len J1 m andS eval_false a.
+  * move => st0 [x [h0 [[h1 h2] h3]]].
+    split => //. split => //.
+    by apply: (Len_monotone2 h0 h2).
+  move: (tsemax2_conseq_R hpost hs) => {hpost}hs.
   have hpost: (J0 andS Len J1 m andS eval_false a) ->>
-  Last ([|w|] *** <<u0>> *** Iter (p *** <<u>>) *** [|eval_false a|])
-  andS Len r m.
-  * move => st0. rewrite /J0. rewrite /J1. move => [h0 [h1 h2]]. split.
-    have h3 : (Last (<< u0 andS w >> *** Iter (p *** << u >>)) andS eval_false a) st0.
-    * by split.
-    have := Last_andS h3 => {h3}. apply Last_monotone.
-    have := assertT_imp_trans (@Append_assoc_L _ _ _). apply.
-    have := assertT_imp_trans _ (@Append_assoc_L _ _ _). apply.
-    apply Append_monotone_L. clear h0 h1 h2. move => tr0 [st1 [h0 h1]].
-    inv h1. inv H3. destruct h0 as [h0 h1]. simpl. exists (Tnil st1).
-    split. exists st1. split => //. apply bisim_reflexive. apply follows_nil => //.
-    exists st1. split => //. apply bisim_reflexive. clear h0.
-    move => tr0 [h0 h3]. apply h1. split => //. rewrite -h0 in h2. clear h1 h0.
+    Last ([|w|] *** <<u0>> *** Iter (p *** <<u>>) *** [|eval_false a|])
+    andS Len r m.
+  * move => st0. rewrite /J0 /J1. move => [h0 [h1 h2]]. split.
+    - have h3 : (Last (<< u0 andS w >> *** Iter (p *** << u >>)) andS eval_false a) st0
+        by split.
+      apply/Last_monotone/(Last_andS h3) => {h3}.
+      apply: (impT_conseq_L (@Append_assoc_L _ _ _)).
+      apply: (impT_conseq_L _ (@Append_assoc_L _ _ _)).
+      apply: Append_monotone_L => {h2} tr0 [st1 [{}h0 {}h1]].
+      inv h1. inv H3. destruct h0 as [h0 h1]. simpl.
+      exists (Tnil st1). split; first by exact: mk_singleton_nil.
+      by apply/follows_nil/mk_dup.
+    move => tr0 [{}h0 h3]. apply h1. split => //. rewrite -h0 in h2. clear h1 h0.
     destruct r as [r hr]. destruct p as [p hp]. simpl. simpl in h3.
-    exists (Tnil (hd tr0)). split. apply iter_stop. apply follows_nil => //.
-    exists (Tnil (hd tr0)). split. exists (hd (tr0)). split => //.
-    apply bisim_reflexive. apply follows_nil => //.
+    exists (Tnil (hd tr0)). split; first by exact: iter_stop.
+    apply follows_nil => //. exists (Tnil (hd tr0)). split; first by exact: mk_singleton_nil.
+    by exact: follows_nil.
   by apply: (tsemax2_conseq_R hpost hs).
 
-- move => m w r hafter. have h: after ([|w|] *** p2) r.
-  have := after_monotone_L _ hafter. apply. by apply Append_monotone.
-  have := IHsemax m _ _ h => {hafter h IHsemax}. move => htsemax.
-  have := tsemax2_conseq _ _ htsemax => {htsemax}. apply.
-  * move => st0 [h0 [h1 h2]]. split => //. have := H _ h0. done.
-    split => //. have := Len_monotone _ h2. apply. by apply Append_monotone_L.
-  * move => st0 [h0 h1]. split => //. have := Last_monotone _ h0. apply.
-    by apply Append_monotone_R.
+- move => m w r hafter.
+  have h: after ([|w|] *** p2) r
+    by apply/(after_monotone_L _ hafter)/Append_monotone.
+  move: (IHsemax m _ _ h) => {hafter h IHsemax}htsemax.
+  apply: (tsemax2_conseq _ _ htsemax) => {htsemax}.
+  * move => st0 [h0 [h1 h2]]. split; first by apply: H.
+    split => //. by apply/Len_monotone/h2/Append_monotone_L.
+  move => st0 [h0 h1]. split => //.
+  by apply/Last_monotone/h0/Append_monotone_R.
 
 - move => m w r hafter.
   have hsemax: forall x, tsemax2 (u x andS w andS Len (p x *** r) m) s
       (Last (([|w|]) *** p x) andS Len r m).
-  * move => x. apply H0. move hp: (p x) => q. destruct q as [q hq].
-    destruct r as [r hr]. move => tr0 h0. destruct h0 as [tr1 [h0 h1]].
-    have: satisfy ([|w|] *** exT p) tr0. simpl. exists tr1. split => //. clear h0.
-    move: tr1 tr0 h1. cofix hcoind. move => tr0 tr1 h0. inv h0. apply follows_nil => //.
-    exists x. rewrite hp. simpl. done. apply follows_delay. have := hcoind _ _ H1. done.
-    move => h2. have := hafter _ h2. done.
-  have := tsemax2_ex hsemax. clear hafter hsemax. move => hsemax.
-  have := tsemax2_conseq _ _ hsemax => {hsemax}. apply.
-  * move => st0 [h0 [h1 h2]]. destruct h0 as [x h0]. exists x. split => //.
-    split => //. move => tr0 [h3 h4]. apply h2. split => //.
-    have := Append_monotone_L _ h4. apply. move => tr1. move hp: (p x) => q.
-    destruct q as [q hq]. simpl. move => h5. exists x. rewrite hp. by simpl.
-  * move => st0 [x [h0 h1]]. split => //. clear h1. move hp: (p x) => q.
+  * move => x. apply H0. move hp: (p x) => q.
+    destruct q as [q hq]. destruct r as [r hr]. move => tr0 [tr1 [h0 h1]].
+    have h2 : satisfy ([|w|] *** exT p) tr0.
+    - simpl. exists tr1. split => // {h0}.
+      move: tr1 tr0 h1. cofix CIH=>tr0 tr1 h0. inv h0.
+      - apply follows_nil => //. exists x. by rewrite hp.
+      by apply/follows_delay/CIH/H1.
+    by exact: hafter _ h2.
+  move: (tsemax2_ex hsemax) => {hafter}hsemax.
+  apply: (tsemax2_conseq _ _ hsemax) => {hsemax}.
+  * move => st0 [[x h0] [h1 h2]]. exists x.
+    split => //. split => // tr0 [h3 h4]. apply h2. split => //.
+    apply: (Append_monotone_L _ h4) => tr1. move hp: (p x) => [q hq] /= h5.
+    exists x. by rewrite hp.
+  * move => st0 [x [h0 h1]]. split => // {h1}. move hp: (p x) => q.
     rewrite hp in h0. destruct q as [q hq]. destruct h0 as [tr0 [h1 h0]].
-    simpl. exists tr0. split => //. clear h0. destruct h1 as [tr1 [h0 h1]].
+    simpl. exists tr0. split => // {h0}. destruct h1 as [tr1 [h0 h1]].
     exists tr1. split => //. destruct h0 as [st1 [h0 h2]]. inv h2. inv h1.
     apply follows_nil => //. exists x. by rewrite hp.
 Qed.
@@ -666,21 +640,22 @@ move => U s P hsemax.
 have h0: (U andS exS (fun m => Len P m)) ->> (exS (fun m => U andS Len P m)).
 - move => st0 [h0 [n h1]]. exists n. by split.
 have h1: (exS (fun (m:nat) => Last P)) ->> (Last P).
-- move => st0 [n hP]. done.
-have := tsemax2_conseq h0 h1 => {h0 h1}. apply.
-apply tsemax2_ex. move => n. have := (@tsemax2_complete _ _ _ hsemax  n ttS ([| ttS |])).
-clear hsemax; move => hsemax.
-have : after (([|ttS|]) *** P) ([|ttS|]).
-- clear hsemax. destruct P as [P hP]. move => tr0 h0. exists tr0. apply follows_ttS.
-move => h0; have := hsemax h0 => {h0 hsemax}; move => hsemax.
-have := (tsemax2_conseq _ _ hsemax) => {hsemax}. apply.
-- move => st0 h0. destruct h0 as [h0 h1]. try (repeat split; auto).
-  move => tr0. clear h0. move => [h0 h2]. have := h1 tr0 => {h1}. apply; split => //.
-  destruct P as [P hP]. simpl in h2. simpl. have := (append_singleton _ h2).
-  by apply.
-- destruct P as [P hP]. simpl. move => st0 [h0 _]. have := (last_cont _ h0).
-  apply. move => tr0 [tr1 [h1 h2]]. destruct h1 as [st1 [_ h1]].
-  inversion h1; subst; clear h1. inversion h2; subst; clear h2. done.
+- by move => st0 [n hP].
+apply: (tsemax2_conseq h0 h1) => {h0 h1}.
+apply tsemax2_ex => n.
+move: (@tsemax2_complete _ _ _ hsemax  n ttS ([| ttS |])) => {}hsemax.
+have h0 : after (([|ttS|]) *** P) ([|ttS|]).
+- clear hsemax. destruct P as [P hP]. move => tr0 h0. exists tr0. by apply follows_ttS.
+move: (hsemax h0) => {h0}hsemax.
+apply: (tsemax2_conseq _ _ hsemax) => {hsemax}.
+- move => st0 h0. destruct h0 as [h0 h1]. do!split=>//.
+  move => tr0 [{}h0 h2].
+  apply: (h1 tr0) => {h1}; split => //.
+  destruct P as [P hP]. simpl in h2. simpl.
+  by apply: (append_singleton _ h2).
+- destruct P as [P hP]. move => /= st0 [h0 _].
+  apply: (last_cont _ h0) => tr0 [tr1 [[st1 [_ h1]] h2]].
+  inv h1. by inv h2.
 Qed.
 
 Inductive tsemax : assertS -> stmt -> assertS -> Prop :=
@@ -715,14 +690,14 @@ Lemma tsemax_conseq_L: forall s u1 u2 v,
  u1 ->> u2 -> tsemax u2 s v -> tsemax u1 s v.
 Proof.
 move => s u1 u2 v h0 h1.
-exact: (tsemax_conseq h0 (@assertS_imp_refl _) h1).
+by apply/tsemax_conseq/h1.
 Qed.
 
 Lemma tsemax_conseq_R: forall s u v1 v2,
  v2 ->> v1 -> tsemax u s v2 -> tsemax u s v1.
 Proof.
 move => s u v1 v2 h0 h1.
-exact: (tsemax_conseq (@assertS_imp_refl _) h0 h1).
+by exact/tsemax_conseq/h1.
 Qed.
 
 (* Proposition 4.2: embedding the total-correctness Hoare logic into
@@ -732,27 +707,22 @@ Lemma tsemax_correct_semax: forall u s v, tsemax u s v ->
 Proof.
 induction 1.
 - move => u0.
-  have h0 := semax_skip (u andS u0).
-  have h1: [|u andS u0 |] =>> ([|u0|] *** Finite *** [|u|]).
-  * clear h0. move => tr0 [st0 [h0 h1]]. inv h1. move: h0 => [h0 h1].
-    exists (Tnil st0). split. exists st0. split; [done | apply bisim_reflexive].
-    apply follows_nil => //. exists (Tnil st0). split.
-    apply finite_nil. apply follows_nil => //. exists st0.
-    split; [done | apply bisim_reflexive].
-  by apply: (semax_conseq_R h1 h0).
+  apply/semax_conseq_R/(semax_skip (u andS u0)).
+  move => tr0 [st0 [[{}h0 h2] h1]]. inv h1.
+  exists (Tnil st0). split; first by exact: mk_singleton_nil.
+  apply follows_nil => //. exists (Tnil st0). split; first by exact: finite_nil.
+  by apply/follows_nil/mk_singleton_nil.
 - move => u0.
-  have h0 := semax_assign (u andS u0) x a.
-  have h1: (Updt (u andS u0) x a) =>> ([|u0|] *** Finite *** [|udt u x a|]).
-  * move => tr0 [st0 [{}h0 h1]]. inv h1. inv H1.
-    move: h0 => [h0 h1]. exists (Tnil st0). split; first by apply: (mk_singleton_nil h1).
-    apply follows_nil => //. exists (Tcons st0 (Tnil (update x (a st0) st0))).
-    split; first by apply/finite_delay/finite_nil.
-    apply/follows_delay/follows_nil=>//. exists (update x (a st0) st0).
-    split; last by apply: bisim_nil. exists st0. by split.
-  by apply: (semax_conseq_R h1 h0).
+  apply/semax_conseq_R/(semax_assign (u andS u0)).
+  move => tr0 [st0 [[{}h0 h2] h1]]. inv h1. inv H1.
+  exists (Tnil st0). split; first by exact: mk_singleton_nil.
+  apply follows_nil => //. exists (Tcons st0 (Tnil (update x (a st0) st0))).
+  split; first by apply/finite_delay/finite_nil.
+  apply/follows_delay/follows_nil=>//. exists (update x (a st0) st0).
+  split; last by apply: bisim_nil. exists st0. by split.
 - move => u0.
   have h0 := semax_conseq_R (@Append_assoc_R _ _ _) (IHtsemax1 u0) => {IHtsemax1}.
-  have h: u2 ->> (u2 andS u2); first done.
+  have h: u2 ->> (u2 andS u2) by [].
   have h1 := semax_seq h0 (semax_conseq_L h (IHtsemax2 u2)) => {h h0 IHtsemax2}.
   have h0: ((([|u0|]) *** Finite) *** ([|u2|]) *** Finite *** ([|u3|]))
   =>> (([|u0|]) *** Finite *** ([|u3|])).
@@ -762,20 +732,19 @@ induction 1.
     have h1 := Append_assoc_R h0 => {h0}.
     have h0 := Append_assoc_R h1 => {h1}.
     apply: (Append_monotone_L _ h0) => {h0}.
-    apply: (assertT_imp_trans (Append_monotone_L (@Finite_singleton u2))).
+    apply: (impT_conseq_L (Append_monotone_L (@Finite_singleton u2))).
     by apply: Finite_idem_1.
   by apply: (semax_conseq_R h0 h1).
 - move => u0.
   have h: ((u1 andS u0) andS eval_true a) ->> (u1 andS eval_true a) andS u0
-    by move => st0 [[h0 h1] h2]; split; [split| ].
+    by move => st0 [[h0 h1] h2]; do!split.
   have h0: ((u1 andS u0) andS eval_false a) ->> (u1 andS eval_false a) andS u0
-    by move => st0 [[h0 h1] h2]; split; [ split| ].
+    by move => st0 [[h0 h1] h2]; do!split.
   apply: (semax_conseq _ _
             (semax_ifthenelse (semax_conseq_L h (IHtsemax1 u0))
             (semax_conseq_L h0 (IHtsemax2 u0)))) => {h h0 IHtsemax1 IHtsemax2}=>//.
   move => tr0 [tr1 [[st0 [h0 h2]] h1]]. inv h2.
-  inv H3. inv h1. exists (Tnil st0). split.
-  * move: h0 => [_ h0]. by apply: (mk_singleton_nil h0).
+  inv H3. inv h1. exists (Tnil st0). split; first by move: h0=>[_ h0]; apply: mk_singleton_nil.
   inv H4. clear h0.
   move: H3 => [tr0 [[st0 [h0 h2]] h1]]. inv h2. inv h1.
   clear h0. apply follows_nil => //. move: H3 => [tr0 [h0 h1]].
@@ -797,7 +766,7 @@ induction 1.
     by move => n; apply: H0.
   have h0 := semax_ex h => {H0 h}.
   have h1 : (u andS eval_true a) ->> (exS (fun n : nat =>
-  (eval_true a andS u andS (fun st : state => t st = n)) andS (fun st => t st = n))).
+    (eval_true a andS u andS (fun st : state => t st = n)) andS (fun st => t st = n))).
   * move => st0 [{}h0 h1]. exists (t st0). by split.
   have h2 := semax_conseq_L h1 h0 => {h1 h0}.
   have h0:(exT (fun n : nat =>
@@ -806,16 +775,16 @@ induction 1.
   ((exT (fun n: nat =>
    [| (fun st: state => t st = n) |] *** Finite ***
    [| (fun st: state => t st < n) |])) *** [|u|]).
-  * clear h2. move => tr0 [x h0]. move: h0 => [tr1 [h0 h1]].
-    move: h0 => [st0 [h2 h0]]. inv h0. inv h1. move: H1 => [tr1 [h0 h1]].
+  * move => {h2} tr0 [x [tr1 [[st0 [h2 h0]] h1]]].
+    inv h0. inv h1. move: H1 => [tr1 [h0 h1]].
     have h3 := follows_singleton h1.
     have h4 := finite_setoid h0 h3 => {h0}.
-    have h0 := follows_setoid_L h1 h3 => {h3 h1}. exists tr0.
+    have h0 := follows_setoid_L h1 h3 => {h3 h1}.
+    exists tr0.
     have h5 := follows_singleton_andS_R h0.
     have h6 := follows_singleton_andS_L h0 => {h0}.
-    split; last done. exists (t (hd tr0)). exists (Tnil (hd tr0)). split.
-    exists (hd tr0). split; [done | apply bisim_reflexive]. apply follows_nil => //.
-    exists tr0. by split.
+    split=>//. exists (t (hd tr0)). exists (Tnil (hd tr0)). split; first by exact: mk_singleton_nil.
+    apply follows_nil => //. by exists tr0.
   have h1 := semax_conseq_R h0 h2 => {h0 h2}.
   have h: (u andS u0) ->> u.  move => st [h0 h2]; done.
   have h0 := semax_while h h1 => { h h1}.
@@ -827,70 +796,70 @@ induction 1.
               Finite *** ([|fun st : state => t st < n|])) *** (<< u >>)) ***
         ([|eval_false a|])) =>>
   (([|u0 |]) *** Finite *** ([|u andS eval_false a|])).
-  * clear h0. move => tr0 [tr1 [h0 h1]]. move: h0 => [st0 [[h0 h] h2]].
-    inv h2. inv H1. inv h1. inv H2. exists (Tnil (hd tr')). split. exists (hd tr').
-    split; [done | apply bisim_reflexive]. apply follows_nil => //.
+  * move => tr0 [tr1 [[st0 [[{}h0 h] h2]] h1]].
+    inv h2. inv H1. inv h1. inv H2.
+    exists (Tnil (hd tr')). split; first by exact: mk_singleton_nil.
+    apply follows_nil => //.
     move: H1 => [tr0 [h1 h2]]. exists (Tcons (hd tr') tr'). split; first last.
-    apply follows_delay. apply singleton_andS_follows; first last.
-    have h3 := follows_singleton h2.
-    have h4 := follows_setoid (@singleton_setoid _) h2 h3 (bisim_reflexive _) => {h2 h3}.
-    by apply h4. have h4 := follows_singleton h2.
-    have := follows_setoid (@singleton_setoid  _) _ h4 h4 => {h4}. apply.
-    have h3 := follows_hd h2 => {h2}. rewrite -h3 in h0 => {h3}.
-    have := iter_append_dup h0 h1. by apply. apply finite_delay.
-    clear h0. have h0 := follows_singleton h2 => {h2}.
-    have := finite_setoid _ h0 => {h0}. apply. inv h1. apply finite_nil.
-    move: H => [tr1 [h0 h1]]. move: h0 => [n [tr2 [h0 h2]]].
-    move: h0 => [st0 [h0 h3]]. inv h3. inv h2.
-    move h0: (t (hd tr1)) => n. rewrite h0 in H2. clear h0.  clear h tr'.
+    - apply/follows_delay/singleton_andS_follows; first last.
+      - have h3 := follows_singleton h2.
+        by apply: (follows_setoid (@singleton_setoid _) h2 h3 (bisim_reflexive _)).
+      have h4 := follows_singleton h2.
+      apply: (follows_setoid (@singleton_setoid  _) _ h4 h4) => {h4}.
+      have h3 := follows_hd h2 => {h2}. rewrite -h3 in h0 => {h3}.
+      by apply: (iter_append_dup h0 h1).
+    apply finite_delay.
+    have {}h0 := follows_singleton h2 => {h2}.
+    apply: (finite_setoid _ h0) => {h0}.
+    inv h1; first by exact: finite_nil.
+    move: H => [tr1 [[n [tr2 [[st0 [h0 h3]] h2]]] h1]]. inv h3. inv h2.
+    move h0: (t (hd tr1)) => n. rewrite h0 in H2. clear h0 h tr'.
     have h: forall (m: nat) (n : nat) (tr1 tr tr0 : trace),
-    n <= m ->
-    append (fun tr2 : trace => finite tr2)
-    (singleton (fun st : state => t st < n)) tr1 ->
-    follows (dup u) tr1 tr ->
-    follows
-    (iter
-     (append
-        (fun tr2 : trace =>
-         exists x : nat,
-         satisfy
-           (([|fun st : state => t st = x|]) ***
-            Finite *** ([|fun st : state => t st < x|])) tr2) (dup u))) tr
-    tr0 -> finite tr0. clear tr0 tr H0 tr1 h1 n H2.
-    move => m. induction m.
-    - move => n tr0 tr1 tr2 h h1 h2 h3.
-      have h4: n = 0; first by lia. rewrite h4 in h1 => {h4 h}.
-      move: h1 => [tr3 [h1 h4]].
-      move: tr3 h1 tr0 tr1 tr2 h2 h3 h4. induction 1.
-      - move => tr0 tr1 tr2 h0 h1 h2. inv h2. move: H1 => [st0 [h3 h4]].
-        by inversion h3.
-      - move => tr0 tr1 tr2 h0 h2 h3. inv h3. inv h0.
-        inv h2. apply finite_delay.
-        by apply: (IHh1 _ _ _ H3 H4 H2).
-    - move => n tr0 tr1 tr2 h [tr3 [h0 h3]] h1 h2.
-      move: tr3 h0 tr0 tr1 tr2 h3 h1 h2. induction 1.
-      - move => tr0 tr1 tr2 h0 h1 h2. inv h0. move: H1 => [st0 [h0 h3]].
-        inv h3. inv h1. move: H1 => [st0 [h1 h3]]. inv h3. inv H1. simpl in h0.
-        inv h2. inv H2. apply finite_delay. inv H1. apply finite_nil.
-        move: H => [tr0 [h2 h3]]. move: h2 =>[n0 [tr1 [h2 h4]]].
-        move: h2 => [st0 [h2 h5]]. inv h5. inv h4.
-        rewrite -(follows_hd H0) -(follows_hd h3) in h0.
-        have h2: t (hd tr0) <= m by lia. clear h0.
-        apply: (IHm _ _ _ _ h2 H2 h3 H0).
-    - clear IHm. move => tr0 tr1 tr2 h3 h1 h2. inv h3. inv h1. inv h2.
-      apply finite_delay. by apply: (IHh0 _ _ _ H2 H3 H4).
-    by apply: (h n _ _ _ _ _ H2 h1 H0).
+      n <= m ->
+      append (fun tr2 : trace => finite tr2)
+      (singleton (fun st : state => t st < n)) tr1 ->
+      follows (dup u) tr1 tr ->
+      follows
+      (iter
+       (append
+          (fun tr2 : trace =>
+           exists x : nat,
+           satisfy
+             (([|fun st : state => t st = x|]) ***
+              Finite *** ([|fun st : state => t st < x|])) tr2) (dup u))) tr
+      tr0 -> finite tr0.
+    * move => {tr0 tr H0 tr1 h1 n H2}m. induction m.
+      - move => n tr0 tr1 tr2 h h1 h2 h3.
+        have h4: n = 0 by lia.
+        rewrite h4 in h1 => {h4 h}.
+        move: h1 => [tr3 [h1 h4]].
+        move: tr3 h1 tr0 tr1 tr2 h2 h3 h4. induction 1.
+        - move => tr0 tr1 tr2 h0 h1 h2. inv h2. move: H1 => [st0 [h3 h4]].
+          by inversion h3.
+        - move => tr0 tr1 tr2 h0 h2 h3. inv h3. inv h0.
+          inv h2.
+          by apply/finite_delay/IHh1/H2/H4.
+      - move => n tr0 tr1 tr2 h [tr3 [h0 h3]] h1 h2.
+        move: tr3 h0 tr0 tr1 tr2 h3 h1 h2. induction 1.
+        - move => tr0 tr1 tr2 h0 h1 h2. inv h0. move: H1 => [st0 [h0 h3]].
+          inv h3. inv h1. move: H1 => [st0 [h1 h3]]. inv h3. inv H1. simpl in h0.
+          inv h2. inv H2. apply finite_delay. inv H1. apply finite_nil.
+          move: H => [tr0 [[n0 [tr1 [[st0 [h2 h5]] h4]]] h3]]. inv h5. inv h4.
+          rewrite -(follows_hd H0) -(follows_hd h3) in h0.
+          have h2: t (hd tr0) <= m by lia. clear h0.
+          by apply: (IHm _ _ _ _ h2 H2 h3 H0).
+        - move => {IHm} tr0 tr1 tr2 h3 h1 h2. inv h3. inv h1. inv h2.
+          by apply/finite_delay/IHh0/H4/H3.
+      by apply: (h n _ _ _ _ _ H2 h1 H0).
   by apply: (semax_conseq_R h1 h0).
-- clear H1. move => u0.
+- move => {H1}u0.
   have h0 := IHtsemax u0 => {IHtsemax}.
   apply: (semax_conseq _ _ h0).
-  * clear h0. move => st0 [h0 h1]. by split=>//; apply: H.
-  * clear h0. move => tr0 [tr1 [[st0 [h0 h2]] h1]].
-    inv h2. inv h1. exists (Tnil (hd tr0)). split.
-    + exists (hd tr0). by split=>//; apply bisim_reflexive.
-    apply follows_nil => //.
-    clear h0. move: H3 => [tr1 [h0 h1]]. exists tr1. split=>//.
-    by apply: (follows_monotone (singleton_monotone _) h1).
+  * move => st0 [{}h0 h1]. by split=>//; apply: H.
+  move => tr0 [tr1 [[st0 [{}h0 h2]] h1]].
+  inv h2. inv h1. exists (Tnil (hd tr0)). split; first by exact: mk_singleton_nil.
+  apply follows_nil => // {h0}. move: H3 => [tr1 [h0 h1]]. exists tr1. split=>//.
+  by apply: (follows_monotone (singleton_monotone _) h1).
 Qed.
 
 (* Corollary 4.1 *)
@@ -900,7 +869,7 @@ Proof.
 move => s U V htsemax.
 move: (tsemax_correct_semax htsemax ttS) => {}htsemax.
 apply: (semax_conseq _ _  htsemax); first by move=> st0 hU; split.
-apply: (assertT_imp_trans (@Append_assoc_R _ _ _)).
+apply: (impT_conseq_L (@Append_assoc_R _ _ _)).
 apply: Append_monotone_L => tr [tr1 [[st0 [h0 h2]] h1]].
 by inv h1; inv h2.
 Qed.
