theories/Semax.v
@@ -36,90 +36,62 @@ Inductive semax : assertS -> stmt -> assertT -> Prop :=
   semax (exS u) s (exT p).
 
 Lemma semax_conseq_R: forall u s p q,
-p =>> q -> semax u s p -> semax u s q.
-Proof.
-move => u s p q h0 h1.
-by apply: (semax_conseq (@assertS_imp_refl u) h0 h1).
-Qed.
+  p =>> q -> semax u s p -> semax u s q.
+Proof. move => u s p q h0 h1. by apply/semax_conseq/h1. Qed.
 
 Lemma semax_conseq_L: forall u v s p,
 v ->> u -> semax u s p -> semax v s p.
-Proof.
-move => u v s p h0 h1.
-by apply: (semax_conseq h0 _ h1).
+Proof. move => u v s p h0 h1. by apply/semax_conseq/h1. Qed.
+
+Lemma push_pre_andS: forall u s p, semax u s p -> forall v, semax (u andS v) s ([|v|] *** p).
+induction 1=>v0.
+- apply/semax_conseq_R/semax_skip.
+  apply/impT_conseq_L/Sglt_Chop_2/singleton_monotone.
+  by exact: andS_comm.
+- apply/semax_conseq_R/semax_assign.
+  move => tr0 /= [st0][[h0 h1] h2]. inv h2. inv H1.
+  exists (Tnil st0). split; first by exact: mk_singleton_nil.
+  by apply/follows_nil/mk_updt.
+- move: (semax_conseq_R (@Append_assoc_R _ _ _) (IHsemax1 v0)) => {IHsemax1}hs1.
+  apply/semax_conseq_R/(semax_seq hs1)/semax_conseq_L/IHsemax2/v=>//.
+  by apply/impT_conseq_L/Append_assoc_L/Append_monotone_R/Singleton_Append.
+- have h0: ((u andS v0) andS eval_true a) ->> ((u andS eval_true a) andS v0)
+    by move => st0 [[h0 h1] h2].
+  move: (semax_conseq_L h0 (IHsemax1 v0)) => {h0 IHsemax1}hs1.
+  have h0: ((u andS v0) andS eval_false a) ->> ((u andS eval_false a) andS v0)
+    by move => st0 [[h0 h1] h2].
+  move: (semax_conseq_L h0 (IHsemax2 v0)) => {IHsemax2}hs2.
+  move: (semax_ifthenelse hs1 hs2) => {h0 hs1 hs2}h.
+  apply: (semax_conseq_R _ h).
+  apply: (impT_conseq_L (@Append_assoc_R _ _ _)).
+  apply/impT_conseq_L/Append_assoc_L/Append_monotone_L.
+  move => tr0 /= [tr1][[st0][[h0 h2] h3] h1].
+  inv h3. inv H3. inv h1. inv H4.
+  destruct H3 as [st0 [h1 h3]]. inv h3. simpl in h0. simpl in h2. simpl.
+  exists (Tnil st0). split; first by exact: mk_singleton_nil.
+  by apply/follows_nil/mk_dup.
+- apply/semax_conseq_R/semax_while/H0.
+  * apply/impT_conseq_L/Append_assoc_L/Append_monotone_L.
+    apply/impT_conseq_L/Sglt_Dup_2/Dup_monotone.
+    by exact: andS_comm.
+  by apply: (impS_conseq_L _ H); exact: andS_left.
+- apply/semax_conseq/IHsemax/v0/Append_monotone_R=>//.
+  by apply/(andS_cont H).
+- have hpre: (exS u andS v0) ->> exS (fun x => u x andS v0)
+    by move => st0 [[x h0] h1]; exists x.
+  have hpost: (exT (fun x => [|v0|] *** p x)) =>> ([|v0|] *** exT p).
+  * move => tr0 [x h0]. move hp: (p x) => px. rewrite hp in h0.
+    destruct px as [q hq]. simpl in h0.
+    destruct h0 as [tr1 [[st0 [h0 h2]] h1]].
+    inv h2. inv h1=>/=.
+    exists (Tnil (hd tr0)). split; first by exact: mk_singleton_nil.
+    apply follows_nil => //. exists x. by rewrite hp.
+  apply: (semax_conseq hpre hpost). apply: semax_ex => {hpre hpost}x.
+  by apply: H0.
 Qed.
 
 (* Lemma 3.5 *)
 Lemma push_pre: forall u s p, semax u s p -> semax u s ([|u|] *** p).
 Proof.
-have: forall u s p, semax u s p -> forall v, semax (u andS v) s ([|v|] *** p).
-induction 1.
-- move=>v; apply: (semax_conseq_R _ (semax_skip _)).
-  move=>tr0 /= [st0 [h0 h1]]. inv h1. exists (Tnil st0).
-  move: h0=>[h0 h1]. split.
-  - exists st0. by split=>//; apply: bisim_reflexive.
-  apply follows_nil => //. exists st0. by split => //; apply: bisim_reflexive.
-- move => v. apply: (semax_conseq_R _ (semax_assign _ _ _)).
-  move => tr0 /= [st0 [h0 h1]]. inv h1. inv H1.
-  move: h0=>[h0 h1]. exists (Tnil st0). split.
-  - exists st0. by split => //; apply bisim_reflexive.
-  apply follows_nil => //. exists st0.
-  by split => //; apply: bisim_reflexive.
-- move => v0.
-  have hs1 := IHsemax1 v0 => {IHsemax1}.
-  have hs2 := IHsemax2 v => {IHsemax2}.
-  move: (semax_conseq_R (@Append_assoc_R _ _ _) hs1) => {}hs1.
-  apply: (semax_conseq_R _ (semax_seq hs1 (semax_conseq_L _ hs2))) => //.
-  apply: (assertT_imp_trans _ (@Append_assoc_L _ _ _)).
-  by apply/Append_monotone_R/Singleton_Append.
-- move => v.
-  have hs1 := IHsemax1 v => {IHsemax1}.
-  have h0: ((u andS v) andS eval_true a) ->> ((u andS eval_true a) andS v)
-    by move => st0 [[h0 h1] h2].
-  move: (semax_conseq_L h0 hs1) => {}hs1.
-  have hs2 := IHsemax2 v => {IHsemax2 h0}.
-  have h0: ((u andS v) andS eval_false a) ->> ((u andS eval_false a) andS v)
-   by move => st0 [[h0 h1] h2].
-  move: (semax_conseq_L h0 hs2) => {}hs2.
-  move: (semax_ifthenelse hs1 hs2) => {h0 hs1 hs2}h.
-  apply: (semax_conseq_R _ h).
-  apply: (assertT_imp_trans (@Append_assoc_R _ _ _)).
-  apply: (assertT_imp_trans _ (@Append_assoc_L _ _ _)).
-  apply: Append_monotone_L => tr0 /= [tr1 [h0 h1]].
-  move: h0 => [st0 [h0 h2]]. inv h2. inv H3. move: h0 => [h0 h2].
-  inv h1. inv H4. destruct H3 as [st0 [h1 h3]]. inv h3. simpl in h0. simpl in h2.
-  simpl. exists (Tnil st0). split; first by exists st0; split => //; apply: bisim_reflexive.
-  apply follows_nil => //. exists st0. by split => //; apply: bisim_reflexive.
-- move => v.
-  move: (IHsemax ttS) => {IHsemax}hs.
-  have hpre: (u andS eval_true a) ->> (u andS eval_true a) andS ttS
-    by move => st0 [h0 h1]; split.
-  move: (semax_conseq_L hpre hs) => {hpre}hs.
-  move: (semax_conseq_R (@ttS_Chop _) hs) => {}hs.
-  apply: (semax_conseq_R _ (semax_while _ hs)).
-  * apply: (assertT_imp_trans _ (@Append_assoc_L _ _ _)).
-    apply: Append_monotone_L => tr0 [st0 [[h0 h2] h1]].
-    inv h1. inv H3. simpl. exists (Tnil st0). split.
-    + exists st0. by split => //; apply: bisim_reflexive.
-    apply follows_nil => //. exists st0. by split => //; apply bisim_reflexive.
-  move => st0 [h0 h1]. by apply: H.
-- move => v.
-  have hs := IHsemax v => {IHsemax}.
-  apply: (semax_conseq _ _ hs).
-  * move => st0 [h0 h1]. split => //. by apply: H.
-  by apply Append_monotone_R.
-- move => v.
-  have hpre: (exS u andS v) ->> exS (fun x => u x andS v).
-  * move => st0 [h0 h1]. destruct h0 as [x h0]. by exists x.
-  have hpost: (exT (fun x => [|v|] *** p x)) =>> ([|v|] *** exT p).
-  * move => tr0 [x h0]. move hp: (p x) => px. rewrite hp in h0.
-    destruct px as [q hq]. simpl in h0. destruct h0 as [tr1 [h0 h1]].
-    destruct h0 as [st0 [h0 h2]]. inv h2. inv h1. simpl.
-    exists (Tnil (hd tr0)). split.
-    + exists (hd tr0). by split => //; apply: bisim_reflexive.
-    apply follows_nil => //. exists x. by rewrite hp.
-  apply: (semax_conseq hpre hpost). apply: semax_ex => {hpre hpost}x.
-  by apply: H0.
-move => h u s p hs. move: (h _ _ _ hs) => {}hs.
-by apply: (semax_conseq_L _ (hs _)).
+move => u s p hs. by apply/semax_conseq_L/push_pre_andS/hs.
 Qed.
