theories/SemaxSound.v
@@ -9,31 +9,29 @@ Lemma semax_sound : forall u s p, semax u s p ->
  forall st tr, exec s st tr -> u st -> satisfy p tr.
 Proof.
 induction 1 => st0 tr0 hexec hu.
-- exists st0. inv hexec. by split=>//; apply: bisim_reflexive.
-- inv hexec. exists st0. by split=>//; apply: bisim_reflexive.
+- inv hexec=>/=; by exact: mk_singleton_nil.
+- inv hexec=>/=. by exact: mk_updt.
 - inv hexec.
   have h1 := IHsemax1 _ _ H3 hu.
   destruct p1 as [f1 hf1]. destruct p2 as [f2 hf2].
   clear H H0. simpl in IHsemax1. simpl in IHsemax2. simpl in h1. simpl.
   exists tr. split.
-  * by apply: (@append_singleton f1 hf1 v _ h1).
+  * by apply/(@append_singleton f1)/h1.
   * clear st0 hu H3. move: h1 => [tr1[_ h1]].
      have h0 := follows_singleton h1.
      have h2 := follows_setoid_L h1 h0 => {h0 h1 IHsemax1 tr1}.
      move: tr tr0 h2 H6. cofix CIH=> tr0 tr1 h0 h1. inv h1.
      - inversion h0. clear H3 H1 H0. move: H2 => [st1 [h1 h2]].
         inv h2. have h2 := exec_hd H.
-       apply follows_nil => //. by apply: (IHsemax2 _ _ H h1).
-     - inv h0. by apply: (follows_delay e (CIH _ _ H1 H)).
+       by apply/follows_nil/IHsemax2/h1.
+     - inv h0. by apply/follows_delay/CIH/H.
 - destruct p as [f hf]. exists (Tcons st0 (Tnil st0)). inv hexec.
- * inv H7. inv H5. split.
-  * exists st0. by split=>//; apply: bisim_reflexive.
-  * apply: follows_delay. have h0 := exec_hd H3. apply follows_nil => //.
+ * inv H7. inv H5. split; first by exact: mk_dup.
+  * apply/follows_delay/follows_nil; first by exact: exec_hd H3.
     have h1: (u andS eval_true a) st0 by split.
     by apply: (IHsemax1 _ _ H3 h1).
- * inv H7. inv H5. split.
-   * exists st0. by split=>//; apply: bisim_reflexive.
-   * apply: follows_delay. have h0 := exec_hd H3. apply follows_nil => //.
+ * inv H7. inv H5. split; first by exact: mk_dup.
+   * apply/follows_delay/follows_nil; first by exact: exec_hd H3.
   * have h1: (u andS eval_false a) st0 by split.
     by apply: (IHsemax2 _ _ H3 h1).
 - clear H0. destruct p as [p hp]. simpl in IHsemax. simpl.
@@ -43,8 +41,8 @@ induction 1 => st0 tr0 hexec hu.
     have h: forall tr0 tr1, follows (singleton u) tr0 tr0 -> execseq (Swhile a s) tr0 tr1 ->
     follows (iter (append p (dup u))) (lastdup tr0) tr1.
     + cofix CIH1=>{H st0 hexec hu}tr0 tr1 h0 h1. inv h1.
-      - inversion h0. clear h0 H1 H0 H3. move: H2 => [st1 [h1 h2]]. inv h2.
-        rewrite [lastdup _]trace_destr. simpl. inv H.
+      - inversion h0=>{h0 H1 H0 H3}. move: H2 => [st1 [h1 h2]]. inv h2.
+        rewrite [lastdup _]trace_destr /=. inv H.
         * apply/follows_delay/follows_nil=>//. by apply iter_stop.
       - inversion H3; subst. inversion H5; subst. inversion H6; subst.
         apply/follows_delay/follows_nil.
@@ -73,29 +71,25 @@ induction 1 => st0 tr0 hexec hu.
     have h1: forall tr0 tr1, execseq (Swhile a s) tr0 tr1 ->
     follows (singleton(eval_false a)) tr1 tr1.
     * cofix CIH=> tr0 tr1 h1. inv h1.
-      + inv H0.
-        - apply/follows_delay/follows_nil=>//.
-          exists st. by split; [apply: H5| apply: bisim_reflexive].
+      + inv H0; first by apply/follows_delay/follows_nil/mk_singleton_nil.
         inv H4. inv H6. inv H7.
         by apply: (follows_delay st (CIH _ _ H6)).
       by apply: (follows_delay e (CIH _ _ H0)).
-    move => st0 tr0 h0. inv h0. apply/follows_delay/follows_nil=>//.
-    exists st0. split; [apply: H4|apply: bisim_reflexive].
+    move => st0 tr0 h0.
+    inv h0; first by apply/follows_delay/follows_nil/mk_singleton_nil.
     by apply: (h1 _ _ H6).
   inversion hexec; subst.
-  - exists (Tcons st0 (Tnil st0)). split.
-    * exists st0. by split; [apply: hu| apply: bisim_reflexive].
+  - exists (Tcons st0 (Tnil st0)). split; first by exact: mk_dup.
     apply/follows_delay/follows_nil => //.
     exists (Tnil st0). split; first by apply: iter_stop.
-    apply follows_nil => //. exists st0. by split; [apply: H4| apply: bisim_reflexive].
+    by apply/follows_nil/mk_singleton_nil.
   - inversion H3; subst. inversion H7; subst. inversion H6; subst.
-    exists (Tcons st0 (Tnil st0)). split.
-    * exists st0. by split; [apply hu| apply: bisim_reflexive].
+    exists (Tcons st0 (Tnil st0)). split; first by exact: mk_dup.
     apply/follows_delay/follows_nil => //.
     * rewrite -(exec_hd H4). by apply: (execseq_hd H9).
     exists tr'0. split.
     * by apply: (h0 _ (H _ hu) _ hexec).
-    have h2 := h1 _ _ hexec. inv h2. by apply: H1.
+    have h2 := h1 _ _ hexec. by inv h2.
 - by apply: (H0 _ (IHsemax _ _ hexec (H _ hu))).
 - move: hu => [x h0]. exists x.
   by apply: (H0 _ _ _ hexec h0).
